coq/theories/derivations/AsmToStringDerivations.v
@@ -6,9 +6,10 @@ Require Import impboot.imperative.ImpSyntax.
 Require Import impboot.utils.AppList.
 Require Import impboot.imp2asm.ImpToASMCodegen.
 From impboot Require Import automation.Ltac2Utils.
-From impboot Require Import commons.PrintingUtils.
+From impboot Require Import commons.CompilerUtils.
 From impboot Require Import functional.FunValues.
 From impboot Require Import functional.FunSemantics.
+From impboot Require Import assembly.ASMSyntax.
 Require Import impboot.automation.RelCompiler.
 Require Import impboot.automation.ltac2.UnfoldFix.
 Require Import impboot.automation.AutomationLemmas.
@@ -19,7 +20,7 @@ From Stdlib Require Import derive.Derive.
 From Stdlib Require Import Lia.
 From Ltac2 Require Import Ltac2.
 
-Require Import Patat.Patat.
+From impboot Require Import derivations.CompilerUtilsDerivations.
 
 Set Printing Goal Names.
 Set Printing Existential Instances.
@@ -42,24 +43,8 @@ Proof. unfold_fix_proof 'instrs2str. Qed.
 (* Set Printing Depth 100000. *)
 
 Derive reg2str1_prog
-  in ltac2:(relcompile_tpe 'reg2str1_prog 'reg2str1 ['append])
+  in ltac2:(relcompile_tpe 'reg2str1_prog 'reg2str1 ['string_append])
   as reg2str1_prog_proof.
-Proof.
-  time relcompile.
-Qed.
-
-Derive num2str_f_prog
-  in ltac2:(relcompile_tpe 'num2str_f_prog 'num2str_f ['nat_modulo])
-  as num2str_f_prog_proof.
-Proof.
-  (* when fuel := 0 it compiles `10` as `S (S (... fuel))` *)
-  time relcompile.
-  all: specialize nat_modulo_le with (n := n) (m := 10); ltac1:(lia). 
-Qed.
-
-Derive num2str_prog
-  in ltac2:(relcompile_tpe 'num2str_prog 'num2str ['num2str_f])
-  as num2str_prog_proof.
 Proof.
   time relcompile.
 Qed.
@@ -78,79 +63,165 @@ Proof.
   time relcompile.
 Qed.
 
-Theorem append_equation: ltac2:(unfold_fix_type '@append).
-Proof. unfold_fix_proof '@append. Qed.
-Derive append_prog
-  in ltac2:(relcompile_tpe 'append_prog 'append [])
-  as append_prog_proof.
+Derive inst2str_const_prog
+  in ltac2:(relcompile_tpe 'inst2str_const_prog 'inst2str_const ['reg2str1; 'string_append; 'N2str])
+  as inst2str_const_prog_proof.
 Proof.
   time relcompile.
 Qed.
 
-(* Definition reg2str (r: reg) (str: string): string :=
-  match r with
-  | RAX => "%rax"
-  | RDI => "%rdi"
-  | RBX => "%rbx"
-  | RBP => "%rbp"
-  | R12 => "%r12"
-  | R13 => "%r13"
-  | R14 => "%r14"
-  | R15 => "%r15"
-  | RDX => "%rdx"
-  end ++ str.
-
-Definition str_test (n: nat) (r: reg) (str: string): string :=
-  (reg2str r (num2str n str)).
-
-Opaque name_enc.
-
-Print reg2str.
-Print num2str.
-
-Derive str_test_prog
-  in ltac2:(relcompile_tpe 'str_test_prog 'str_test ['num2str; 'reg2str])
-  as str_test_prog_proof.
+Derive inst2str_mov_prog
+  in ltac2:(relcompile_tpe 'inst2str_mov_prog 'inst2str_mov ['reg2str1; 'string_append])
+  as inst2str_mov_prog_proof.
 Proof.
-  ltac1:(timeout 2 ltac2:(relcompile)). (* fails *)
   time relcompile.
 Qed.
 
-Definition reg2str1 (r: reg) (str: string): string :=
-  match r with
-  | RAX => "%rax"
-  | RDI => "%rdi"
-  | RBX => "%rbx"
-  | RBP => "%rbp"
-  | R12 => "%r12"
-  | R13 => "%r13"
-  | R14 => "%r14"
-  | R15 => "%r15"
-  | RDX => "%rdx"
-  end ++ str.
-
-Definition str_test1 (n: nat) (r: reg) (str: string): string :=
-  (reg2str1 r (num2str n str)).
-
-Opaque name_enc.
-
-Print reg2str1.
-Print num2str.
-
-Derive str_test_prog
-  in ltac2:(relcompile_tpe 'str_test_prog 'str_test1 ['num2str; 'reg2str1])
-  as str_test_prog_proof.
+Derive inst2str_add_prog
+  in ltac2:(relcompile_tpe 'inst2str_add_prog 'inst2str_add ['reg2str1; 'string_append])
+  as inst2str_add_prog_proof.
 Proof.
-  ltac1:(timeout 2 ltac2:(relcompile)). (* succeeds *)
   time relcompile.
-Qed. *)
+Qed.
 
+Derive inst2str_sub_prog
+  in ltac2:(relcompile_tpe 'inst2str_sub_prog 'inst2str_sub ['reg2str1; 'string_append])
+  as inst2str_sub_prog_proof.
+Proof.
+  time relcompile.
+Qed.
+
+Derive inst2str_div_prog
+  in ltac2:(relcompile_tpe 'inst2str_div_prog 'inst2str_div ['reg2str1; 'string_append])
+  as inst2str_div_prog_proof.
+Proof.
+  time relcompile.
+Qed.
+
+Derive inst2str_jump_always_prog
+  in ltac2:(relcompile_tpe 'inst2str_jump_always_prog 'inst2str_jump_always ['reg2str1; 'string_append; 'lab])
+  as inst2str_jump_always_prog_proof.
+Proof.
+  time relcompile.
+Qed.
+
+Derive inst2str_jump_equal_prog
+  in ltac2:(relcompile_tpe 'inst2str_jump_equal_prog 'inst2str_jump_equal ['reg2str1; 'string_append; 'lab])
+  as inst2str_jump_equal_prog_proof.
+Proof.
+  time relcompile.
+Qed.
+
+Derive inst2str_jump_less_prog
+  in ltac2:(relcompile_tpe 'inst2str_jump_less_prog 'inst2str_jump_less ['reg2str1; 'string_append; 'lab])
+  as inst2str_jump_less_prog_proof.
+Proof.
+  time relcompile.
+Qed.
+
+Derive inst2str_call_prog
+  in ltac2:(relcompile_tpe 'inst2str_call_prog 'inst2str_call ['reg2str1; 'string_append; 'lab])
+  as inst2str_call_prog_proof.
+Proof.
+  time relcompile.
+Qed.
+
+Derive inst2str_ret_prog
+  in ltac2:(relcompile_tpe 'inst2str_ret_prog 'inst2str_ret ['reg2str1; 'string_append; 'lab])
+  as inst2str_ret_prog_proof.
+Proof.
+  time relcompile.
+Qed.
+
+Derive inst2str_pop_prog
+  in ltac2:(relcompile_tpe 'inst2str_pop_prog 'inst2str_pop ['reg2str1; 'string_append; 'lab])
+  as inst2str_pop_prog_proof.
+Proof.
+  time relcompile.
+Qed.
+
+Derive inst2str_push_prog
+  in ltac2:(relcompile_tpe 'inst2str_push_prog 'inst2str_push ['reg2str1; 'string_append; 'lab])
+  as inst2str_push_prog_proof.
+Proof.
+  time relcompile.
+Qed.
+
+Derive inst2str_load_rsp_prog
+  in ltac2:(relcompile_tpe 'inst2str_load_rsp_prog 'inst2str_load_rsp ['reg2str1; 'string_append; 'lab; 'mul_nat; 'num2str])
+  as inst2str_load_rsp_prog_proof.
+Proof.
+  time relcompile.
+Qed.
+
+Derive inst2str_store_rsp_prog
+  in ltac2:(relcompile_tpe 'inst2str_store_rsp_prog 'inst2str_store_rsp ['reg2str1; 'string_append; 'lab; 'mul_nat; 'num2str])
+  as inst2str_store_rsp_prog_proof.
+Proof.
+  time relcompile.
+Qed.
+
+Derive inst2str_add_rsp_prog
+  in ltac2:(relcompile_tpe 'inst2str_add_rsp_prog 'inst2str_add_rsp ['reg2str1; 'string_append; 'lab; 'mul_nat; 'num2str])
+  as inst2str_add_rsp_prog_proof.
+Proof.
+  time relcompile.
+Qed.
+
+Derive inst2str_sub_rsp_prog
+  in ltac2:(relcompile_tpe 'inst2str_sub_rsp_prog 'inst2str_sub_rsp ['reg2str1; 'string_append; 'lab; 'mul_nat; 'num2str])
+  as inst2str_sub_rsp_prog_proof.
+Proof.
+  time relcompile.
+Qed.
+
+Derive inst2str_store_prog
+  in ltac2:(relcompile_tpe 'inst2str_store_prog 'inst2str_store ['reg2str1; 'string_append; 'lab; 'mul_nat; 'num2str; 'N2str])
+  as inst2str_store_prog_proof.
+Proof.
+  time relcompile.
+Qed.
+
+Derive inst2str_load_prog
+  in ltac2:(relcompile_tpe 'inst2str_load_prog 'inst2str_load ['reg2str1; 'string_append; 'lab; 'mul_nat; 'num2str; 'N2str])
+  as inst2str_load_prog_proof.
+Proof.
+  time relcompile.
+Qed.
+
+Derive inst2str_getchar1_prog
+  in ltac2:(relcompile_tpe 'inst2str_getchar1_prog 'inst2str_getchar1 ['reg2str1; 'string_append; 'lab; 'mul_nat; 'num2str; 'N2str])
+  as inst2str_getchar1_prog_proof.
+Proof.
+  time relcompile.
+Qed.
+
+Derive inst2str_putchar_prog
+  in ltac2:(relcompile_tpe 'inst2str_putchar_prog 'inst2str_putchar ['reg2str1; 'string_append; 'lab; 'mul_nat; 'num2str; 'N2str])
+  as inst2str_putchar_prog_proof.
+Proof.
+  time relcompile.
+Qed.
+
+Derive inst2str_exit_prog
+  in ltac2:(relcompile_tpe 'inst2str_exit_prog 'inst2str_exit ['reg2str1; 'string_append; 'lab; 'mul_nat; 'num2str; 'N2str])
+  as inst2str_exit_prog_proof.
+Proof.
+  time relcompile.
+Qed.
+
+Derive inst2str_comment_prog
+  in ltac2:(relcompile_tpe 'inst2str_comment_prog 'inst2str_comment ['reg2str1; 'string_append; 'lab; 'mul_nat; 'num2str; 'N2str; 'clean])
+  as inst2str_comment_prog_proof.
+Proof.
+  time relcompile.
+Qed.
 
 Derive inst2str_prog
-  in ltac2:(relcompile_tpe 'inst2str_prog 'inst2str ['reg2str1; 'num2str; 'N2str; 'lab; 'clean; 'append])
+  in ltac2:(relcompile_tpe 'inst2str_prog 'inst2str ['inst2str_const; 'inst2str_mov; 'inst2str_add; 'inst2str_sub; 'inst2str_div; 'inst2str_jump_always; 'inst2str_jump_equal; 'inst2str_jump_less; 'inst2str_call; 'inst2str_ret; 'inst2str_pop; 'inst2str_push; 'inst2str_load_rsp; 'inst2str_store_rsp; 'inst2str_add_rsp; 'inst2str_sub_rsp; 'inst2str_store; 'inst2str_load; 'inst2str_getchar1; 'inst2str_putchar; 'inst2str_exit; 'inst2str_comment])
   as inst2str_prog_proof.
 Proof.
-  (* ltac1:(timeout 10 ltac2:(relcompile)). *)
+  (* ltac1:(timeout 28 ltac2:(relcompile)). *)
   time relcompile.
 Qed.
 
@@ -164,15 +235,399 @@ Qed.
 Theorem concat_strings_equation: ltac2:(unfold_fix_type '@concat_strings).
 Proof. unfold_fix_proof '@concat_strings. Qed.
 Derive concat_strings_prog
-  in ltac2:(relcompile_tpe 'concat_strings_prog 'concat_strings ['append])
+  in ltac2:(relcompile_tpe 'concat_strings_prog 'concat_strings ['string_append])
   as concat_strings_prog_proof.
 Proof.
   time relcompile.
 Qed.
 
+Derive asm2str_header1_prog
+  in ltac2:(relcompile_tpe 'asm2str_header1_prog 'asm2str_header1 ['instrs2str; 'concat_strings; '@list_append; 'string_append])
+  as asm2str_header1_prog_proof.
+Proof.
+  time relcompile.
+Qed.
+
+Derive asm2str_header2_prog
+  in ltac2:(relcompile_tpe 'asm2str_header2_prog 'asm2str_header2 ['instrs2str; 'concat_strings; '@list_append; 'string_append])
+  as asm2str_header2_prog_proof.
+Proof.
+  time relcompile.
+Qed.
+
+Derive asm2str_header3_prog
+  in ltac2:(relcompile_tpe 'asm2str_header3_prog 'asm2str_header3 ['instrs2str; 'concat_strings; '@list_append; 'string_append])
+  as asm2str_header3_prog_proof.
+Proof.
+  time relcompile.
+Qed.
+
 Derive asm2str_prog
-  in ltac2:(relcompile_tpe 'asm2str_prog 'asm2str ['instrs2str; 'concat_strings; 'append])
+  in ltac2:(relcompile_tpe 'asm2str_prog 'asm2str ['instrs2str; 'concat_strings; '@list_append; 'string_append; 'asm2str_header1; 'asm2str_header2; 'asm2str_header3])
   as asm2str_prog_proof.
 Proof.
   time relcompile.
+Qed.
+
+Definition ASMToString_funs := [
+  reg2str1_prog;           (* 0 *)
+  lab_prog;                (* 1 *)
+  clean_prog;              (* 2 *)
+  inst2str_prog;           (* 4 *)
+  instrs2str_prog;         (* 5 *)
+  concat_strings_prog;     (* 6 *)
+  asm2str_prog;            (* 7 *)
+  asm2str_header1_prog;    (* 8 *)
+  asm2str_header2_prog;    (* 9 *)
+  asm2str_header3_prog;    (* 10 *)
+  inst2str_const_prog;     (* 11 *)
+  inst2str_mov_prog;       (* 12 *)
+  inst2str_add_prog;       (* 13 *)
+  inst2str_sub_prog;       (* 14 *)
+  inst2str_div_prog;       (* 15 *)
+  inst2str_jump_always_prog; (* 16 *)
+  inst2str_jump_equal_prog; (* 17 *)
+  inst2str_jump_less_prog; (* 18 *)
+  inst2str_call_prog;      (* 19 *)
+  inst2str_ret_prog;       (* 20 *)
+  inst2str_pop_prog;       (* 21 *)
+  inst2str_push_prog;      (* 22 *)
+  inst2str_load_rsp_prog;  (* 23 *)
+  inst2str_store_rsp_prog; (* 24 *)
+  inst2str_add_rsp_prog;   (* 25 *)
+  inst2str_sub_rsp_prog;   (* 26 *)
+  inst2str_store_prog;     (* 27 *)
+  inst2str_load_prog;      (* 28 *)
+  inst2str_getchar1_prog;  (* 29 *)
+  inst2str_putchar_prog;   (* 30 *)
+  inst2str_exit_prog;      (* 31 *)
+  inst2str_comment_prog    (* 32 *)
+].
+
+Ltac2 assert_eval_app (fname: constr) :=
+  let tpe := gen_eval_app fname () in
+  assert ($tpe).
+
+Ltac2 assert_eval_app_proof (prf: constr) (list_constr: constr) (n: int) :=
+  eapply $prf; eauto; try (reflexivity);
+  try (eapply $list_constr; do n (eapply in_cons); eapply in_eq).
+
+Ltac2 assert_eval_app_by (fname: constr) (prf: constr) (list_constr_hyp: constr) (n: int) :=
+  let tpe := gen_eval_app fname () in
+  assert ($tpe) by (
+    eapply $prf; eauto; try (reflexivity);
+    eapply $list_constr_hyp; do n (eapply in_cons); eapply in_eq
+  ).
+
+Theorem asm2str_thm:
+  ∀ (s: state) (p: asm),
+    (∀ fname args fn,
+      In (FunSyntax.Defun fname args fn) (CompilerUtils_funs) →
+      lookup_fun fname (funs s) = Some (args, fn)) ->
+    (∀ fname args fn,
+      In (FunSyntax.Defun fname args fn) (ASMToString_funs) →
+      lookup_fun fname (funs s) = Some (args, fn)) ->
+    eval_app (name_enc "asm2str") [encode p] s ((encode (asm2str p)), s).
+Proof.
+  intros * Hlookup_fun_utils Hlookup_fun.
+  assert_eval_app_by 'mul_nat 'mul_nat_prog_proof 'Hlookup_fun_utils 0.
+  assert_eval_app_by 'mul_N_f 'mul_N_f_prog_proof 'Hlookup_fun_utils 1.
+  assert_eval_app_by 'mul_N 'mul_N_prog_proof 'Hlookup_fun_utils 2.
+  assert_eval_app_by 'nat_modulo 'nat_modulo_prog_proof 'Hlookup_fun_utils 3.
+  assert_eval_app_by 'N_modulo 'N_modulo_prog_proof 'Hlookup_fun_utils 4.
+  assert_eval_app_by 'num2str_f 'num2str_f_prog_proof 'Hlookup_fun_utils 5.
+  assert_eval_app_by 'num2str 'num2str_prog_proof 'Hlookup_fun_utils 6.
+  assert_eval_app_by 'N2str_f 'N2str_f_prog_proof 'Hlookup_fun_utils 7.
+  assert_eval_app_by 'N2str 'N2str_prog_proof 'Hlookup_fun_utils 8.
+  assert_eval_app_by 'list_length 'list_length_prog_proof 'Hlookup_fun_utils 9.
+  assert_eval_app_by 'list_append 'list_append_prog_proof 'Hlookup_fun_utils 10.
+  assert_eval_app_by 'flatten 'flatten_prog_proof 'Hlookup_fun_utils 11.
+  assert_eval_app_by 'app_list_length 'app_list_length_prog_proof 'Hlookup_fun_utils 12.
+  assert_eval_app_by 'string_append 'string_append_prog_proof 'Hlookup_fun_utils 13.
+  assert_eval_app_by 'mul_nat 'mul_nat_prog_proof 'Hlookup_fun_utils 14.
+
+
+
+  assert_eval_app 'reg2str1.
+  1: {
+    eapply reg2str1_prog_proof; eauto; try reflexivity.
+    eapply Hlookup_fun; do 0 (eapply in_cons); eapply in_eq.
+  }
+  assert_eval_app 'lab.
+  1: {
+    eapply lab_prog_proof; eauto; try reflexivity.
+    eapply Hlookup_fun; do 1 (eapply in_cons); eapply in_eq.
+  }
+  assert_eval_app 'clean.
+  1: {
+    eapply clean_prog_proof; eauto; try reflexivity.
+    eapply Hlookup_fun; do 2 (eapply in_cons); eapply in_eq.
+  }
+  assert_eval_app 'inst2str.
+  1: {
+    eapply inst2str_prog_proof; eauto; try reflexivity.
+    eapply Hlookup_fun; do 4 (eapply in_cons); eapply in_eq.
+  }
+  assert_eval_app 'instrs2str.
+  1: {
+    eapply instrs2str_prog_proof; eauto; try reflexivity.
+    eapply Hlookup_fun; do 5 (eapply in_cons); eapply in_eq.
+  }
+  assert_eval_app 'concat_strings.
+  1: {
+    eapply concat_strings_prog_proof; eauto; try reflexivity.
+    eapply Hlookup_fun; do 6 (eapply in_cons); eapply in_eq.
+  }
+  assert_eval_app 'asm2str.
+  1: {
+    eapply asm2str_prog_proof; eauto; try reflexivity.
+    eapply Hlookup_fun; do 7 (eapply in_cons); eapply in_eq.
+  }
+  assert_eval_app 'asm2str_header1.
+  1: {
+    eapply asm2str_header1_prog_proof; eauto; try reflexivity.
+    eapply Hlookup_fun; do 8 (eapply in_cons); eapply in_eq.
+  }
+  assert_eval_app 'asm2str_header2.
+  1: {
+    eapply asm2str_header2_prog_proof; eauto; try reflexivity.
+    eapply Hlookup_fun; do 9 (eapply in_cons); eapply in_eq.
+  }
+  assert_eval_app 'asm2str_header3.
+  1: {
+    eapply asm2str_header3_prog_proof; eauto; try reflexivity.
+    eapply Hlookup_fun; do 10 (eapply in_cons); eapply in_eq.
+  }
+  assert_eval_app 'inst2str_const.
+  1: {
+    eapply inst2str_const_prog_proof; eauto; try reflexivity.
+    eapply Hlookup_fun; do 11 (eapply in_cons); eapply in_eq.
+  }
+  assert_eval_app 'inst2str_mov.
+  1: {
+    eapply inst2str_mov_prog_proof; eauto; try reflexivity.
+    eapply Hlookup_fun; do 12 (eapply in_cons); eapply in_eq.
+  }
+  assert_eval_app 'inst2str_add.
+  1: {
+    eapply inst2str_add_prog_proof; eauto; try reflexivity.
+    eapply Hlookup_fun; do 13 (eapply in_cons); eapply in_eq.
+  }
+  assert_eval_app 'inst2str_sub.
+  1: {
+    eapply inst2str_sub_prog_proof; eauto; try reflexivity.
+    eapply Hlookup_fun; do 14 (eapply in_cons); eapply in_eq.
+  }
+  assert_eval_app 'inst2str_div.
+  1: {
+    eapply inst2str_div_prog_proof; eauto; try reflexivity.
+    eapply Hlookup_fun; do 15 (eapply in_cons); eapply in_eq.
+  }
+  assert_eval_app 'inst2str_jump_always.
+  1: {
+    eapply inst2str_jump_always_prog_proof; eauto; try reflexivity.
+    eapply Hlookup_fun; do 16 (eapply in_cons); eapply in_eq.
+  }
+  assert_eval_app 'inst2str_jump_equal.
+  1: {
+    eapply inst2str_jump_equal_prog_proof; eauto; try reflexivity.
+    eapply Hlookup_fun; do 17 (eapply in_cons); eapply in_eq.
+  }
+  assert_eval_app 'inst2str_jump_less.
+  1: {
+    eapply inst2str_jump_less_prog_proof; eauto; try reflexivity.
+    eapply Hlookup_fun; do 18 (eapply in_cons); eapply in_eq.
+  }
+  assert_eval_app 'inst2str_call.
+  1: {
+    eapply inst2str_call_prog_proof; eauto; try reflexivity.
+    eapply Hlookup_fun; do 19 (eapply in_cons); eapply in_eq.
+  }
+  assert_eval_app 'inst2str_ret.
+  1: {
+    eapply inst2str_ret_prog_proof; eauto; try reflexivity.
+    eapply Hlookup_fun; do 20 (eapply in_cons); eapply in_eq.
+  }
+  assert_eval_app 'inst2str_pop.
+  1: {
+    eapply inst2str_pop_prog_proof; eauto; try reflexivity.
+    eapply Hlookup_fun; do 21 (eapply in_cons); eapply in_eq.
+  }
+  assert_eval_app 'inst2str_push.
+  1: {
+    eapply inst2str_push_prog_proof; eauto; try reflexivity.
+    eapply Hlookup_fun; do 22 (eapply in_cons); eapply in_eq.
+  }
+  assert_eval_app 'inst2str_load_rsp.
+  1: {
+    eapply inst2str_load_rsp_prog_proof; eauto; try reflexivity.
+    eapply Hlookup_fun; do 23 (eapply in_cons); eapply in_eq.
+  }
+  assert_eval_app 'inst2str_store_rsp.
+  1: {
+    eapply inst2str_store_rsp_prog_proof; eauto; try reflexivity.
+    eapply Hlookup_fun; do 24 (eapply in_cons); eapply in_eq.
+  }
+  assert_eval_app 'inst2str_add_rsp.
+  1: {
+    eapply inst2str_add_rsp_prog_proof; eauto; try reflexivity.
+    eapply Hlookup_fun; do 25 (eapply in_cons); eapply in_eq.
+  }
+  assert_eval_app 'inst2str_sub_rsp.
+  1: {
+    eapply inst2str_sub_rsp_prog_proof; eauto; try reflexivity.
+    eapply Hlookup_fun; do 26 (eapply in_cons); eapply in_eq.
+  }
+  assert_eval_app 'inst2str_store.
+  1: {
+    eapply inst2str_store_prog_proof; eauto; try reflexivity.
+    eapply Hlookup_fun; do 27 (eapply in_cons); eapply in_eq.
+  }
+  assert_eval_app 'inst2str_load.
+  1: {
+    eapply inst2str_load_prog_proof; eauto; try reflexivity.
+    eapply Hlookup_fun; do 28 (eapply in_cons); eapply in_eq.
+  }
+  assert_eval_app 'inst2str_getchar1.
+  1: {
+    eapply inst2str_getchar1_prog_proof; eauto; try reflexivity.
+    eapply Hlookup_fun; do 29 (eapply in_cons); eapply in_eq.
+  }
+  assert_eval_app 'inst2str_putchar.
+  1: {
+    eapply inst2str_putchar_prog_proof; eauto; try reflexivity.
+    eapply Hlookup_fun; do 30 (eapply in_cons); eapply in_eq.
+  }
+  assert_eval_app 'inst2str_exit.
+  1: {
+    eapply inst2str_exit_prog_proof; eauto; try reflexivity.
+    eapply Hlookup_fun; do 31 (eapply in_cons); eapply in_eq.
+  }
+  assert_eval_app 'inst2str_comment.
+  1: {
+    eapply inst2str_comment_prog_proof; eauto; try reflexivity.
+    eapply Hlookup_fun; do 32 (eapply in_cons); eapply in_eq.
+  }
+
+  assert_eval_app '@list_append.
+  1: {
+    eapply list_append_prog_proof; eauto; try reflexivity.
+    eapply Hlookup_fun; do 40 (eapply in_cons); eapply in_eq.
+  }
+  assert_eval_app 'string_append.
+  1: {
+    eapply string_append_prog_proof; eauto; try reflexivity.
+    eapply Hlookup_fun; do 3 (eapply in_cons); eapply in_eq.
+  }
+  assert_eval_app 'mul_N.
+  1: {
+    eapply mul_N_prog_proof; eauto; try reflexivity.
+    2: eapply Hlookup_fun; do 45 (eapply in_cons); eapply in_eq.
+    eapply mul_N_f_prog_proof; eauto; try reflexivity.
+    eapply Hlookup_fun; do 44 (eapply in_cons); eapply in_eq.
+  }
+  assert_eval_app 'mul_nat.
+  1: {
+    eapply mul_nat_prog_proof; eauto; try reflexivity.
+    eapply Hlookup_fun; do 43 (eapply in_cons); eapply in_eq.
+  }
+  assert_eval_app 'num2str.
+  1: {
+    eapply num2str_prog_proof; eauto; try reflexivity.
+    2: eapply Hlookup_fun; do 36 (eapply in_cons); eapply in_eq.
+    eapply num2str_f_prog_proof; eauto; try reflexivity.
+    2: eapply Hlookup_fun; do 35 (eapply in_cons); eapply in_eq.
+    eapply nat_modulo_prog_proof; eauto; try reflexivity.
+    eapply Hlookup_fun; do 33 (eapply in_cons); eapply in_eq.
+  }
+  assert_eval_app 'concat_strings.
+  1: {
+    eapply concat_strings_prog_proof; eauto; try reflexivity.
+    eapply Hlookup_fun; do 6 (eapply in_cons); eapply in_eq.
+  }
+  assert_eval_app 'string_append.
+  1: {
+    eapply string_append_prog_proof; eauto; try reflexivity.
+    eapply Hlookup_fun; do 3 (eapply in_cons); eapply in_eq.
+  }
+  assert_eval_app 'reg2str1.
+  1: {
+    eapply reg2str1_prog_proof; eauto; try reflexivity.
+    eapply Hlookup_fun; do 0 (eapply in_cons); eapply in_eq.
+  }
+  assert_eval_app 'N2str.
+  1: {
+    eapply N2str_prog_proof; eauto; try reflexivity.
+    2: eapply Hlookup_fun; do 38 (eapply in_cons); eapply in_eq.
+    eapply N2str_f_prog_proof; eauto; try reflexivity.
+    2: eapply Hlookup_fun; do 37 (eapply in_cons); eapply in_eq.
+    eapply N_modulo_prog_proof; eauto; try reflexivity.
+    eapply Hlookup_fun; do 34 (eapply in_cons); eapply in_eq.
+  }
+  assert_eval_app 'lab.
+  1: {
+    eapply lab_prog_proof; eauto; try reflexivity.
+    eapply Hlookup_fun; do 1 (eapply in_cons); eapply in_eq.
+  }
+  assert_eval_app 'instrs2str.
+  1: {
+    eapply instrs2str_prog_proof; eauto; try reflexivity.
+    2: eapply Hlookup_fun; do 5 (eapply in_cons); eapply in_eq.
+    eapply inst2str_prog_proof; eauto; try reflexivity.
+    23: eapply Hlookup_fun; do 4 (eapply in_cons); eapply in_eq.
+    1: eapply inst2str_const_prog_proof; eauto; try reflexivity.
+    1: eapply Hlookup_fun; do 11 (eapply in_cons); eapply in_eq.
+    1: eapply inst2str_mov_prog_proof; eauto; try reflexivity.
+    1: eapply Hlookup_fun; do 12 (eapply in_cons); eapply in_eq.
+    1: eapply inst2str_add_prog_proof; eauto; try reflexivity.
+    1: eapply Hlookup_fun; do 13 (eapply in_cons); eapply in_eq.
+    1: eapply inst2str_sub_prog_proof; eauto; try reflexivity.
+    1: eapply Hlookup_fun; do 14 (eapply in_cons); eapply in_eq.
+    1: eapply inst2str_div_prog_proof; eauto; try reflexivity.
+    1: eapply Hlookup_fun; do 15 (eapply in_cons); eapply in_eq.
+    1: eapply inst2str_jump_always_prog_proof; eauto; try reflexivity.
+    1: eapply Hlookup_fun; do 16 (eapply in_cons); eapply in_eq.
+    1: eapply inst2str_jump_equal_prog_proof; eauto; try reflexivity.
+    1: eapply Hlookup_fun; do 17 (eapply in_cons); eapply in_eq.
+    1: eapply inst2str_jump_less_prog_proof; eauto; try reflexivity.
+    1: eapply Hlookup_fun; do 18 (eapply in_cons); eapply in_eq.
+    1: eapply inst2str_call_prog_proof; eauto; try reflexivity.
+    1: eapply Hlookup_fun; do 19 (eapply in_cons); eapply in_eq.
+    1: eapply inst2str_ret_prog_proof; eauto; try reflexivity.
+    1: eapply Hlookup_fun; do 20 (eapply in_cons); eapply in_eq.
+    1: eapply inst2str_pop_prog_proof; eauto; try reflexivity.
+    1: eapply Hlookup_fun; do 21 (eapply in_cons); eapply in_eq.
+    1: eapply inst2str_push_prog_proof; eauto; try reflexivity.
+    1: eapply Hlookup_fun; do 22 (eapply in_cons); eapply in_eq.
+    1: eapply inst2str_load_rsp_prog_proof; eauto; try reflexivity.
+    1: eapply Hlookup_fun; do 23 (eapply in_cons); eapply in_eq.
+    1: eapply inst2str_store_rsp_prog_proof; eauto; try reflexivity.
+    1: eapply Hlookup_fun; do 24 (eapply in_cons); eapply in_eq.
+    1: eapply inst2str_add_rsp_prog_proof; eauto; try reflexivity.
+    1: eapply Hlookup_fun; do 25 (eapply in_cons); eapply in_eq.
+    1: eapply inst2str_sub_rsp_prog_proof; eauto; try reflexivity.
+    1: eapply Hlookup_fun; do 26 (eapply in_cons); eapply in_eq.
+    1: eapply inst2str_store_prog_proof; eauto; try reflexivity.
+    1: eapply Hlookup_fun; do 27 (eapply in_cons); eapply in_eq.
+    1: eapply inst2str_load_prog_proof; eauto; try reflexivity.
+    1: eapply Hlookup_fun; do 28 (eapply in_cons); eapply in_eq.
+    1: eapply inst2str_getchar1_prog_proof; eauto; try reflexivity.
+    1: eapply Hlookup_fun; do 29 (eapply in_cons); eapply in_eq.
+    1: eapply inst2str_putchar_prog_proof; eauto; try reflexivity.
+    1: eapply Hlookup_fun; do 30 (eapply in_cons); eapply in_eq.
+    1: eapply inst2str_exit_prog_proof; eauto; try reflexivity.
+    1: eapply Hlookup_fun; do 31 (eapply in_cons); eapply in_eq.
+    eapply inst2str_comment_prog_proof; eauto; try reflexivity.
+    2: eapply Hlookup_fun; do 32 (eapply in_cons); eapply in_eq.
+    eapply clean_prog_proof; eauto; try reflexivity.
+    eapply Hlookup_fun; do 2 (eapply in_cons); eapply in_eq.
+  }
+  eapply asm2str_prog_proof; eauto; try reflexivity.
+  4: eapply Hlookup_fun; do 7 (eapply in_cons); eapply in_eq.
+  1: eapply asm2str_header1_prog_proof; eauto; try reflexivity.
+  1: eapply Hlookup_fun; do 8 (eapply in_cons); eapply in_eq.
+  1: eapply asm2str_header2_prog_proof; eauto; try reflexivity.
+  1: eapply Hlookup_fun; do 9 (eapply in_cons); eapply in_eq.
+  eapply asm2str_header3_prog_proof; eauto; try reflexivity.
+  eapply Hlookup_fun; do 10 (eapply in_cons); eapply in_eq.
 Qed.
