coq/theories/derivations/ImpToASMCodegenDerivations.v
@@ -5,13 +5,15 @@ Require Import impboot.assembly.ASMToString.
 Require Import impboot.imperative.ImpSyntax.
 Require Import impboot.utils.AppList.
 Require Import impboot.imp2asm.ImpToASMCodegen.
+Require Import impboot.commons.CompilerUtils.
 From impboot Require Import automation.Ltac2Utils.
 From impboot Require Import functional.FunValues.
 From impboot Require Import functional.FunSemantics.
 Require Import impboot.automation.RelCompiler.
 Require Import impboot.automation.ltac2.UnfoldFix.
+Require Import impboot.automation.Ltac2Utils.
 Require Import impboot.automation.AutomationLemmas.
-Require Import impboot.commons.PrintingUtils.
+Require Import impboot.commons.CompilerUtils.
 Require Import coqutil.Word.Interface.
 Require Import ZArith.
 From Stdlib Require Import FunInd.
@@ -26,6 +28,8 @@ Set Printing Existential Instances.
 
 Open Scope app_list_scope.
 
+From impboot Require Import derivations.CompilerUtilsDerivations.
+
 (* *********************************************** *)
 (*       Derivations for Codegen Functions         *)
 (* *********************************************** *)
@@ -34,7 +38,7 @@ Opaque encode.
 Opaque name_enc.
 
 Derive init_prog
-  in ltac2:(relcompile_tpe 'init_prog 'init []) 
+  in ltac2:(relcompile_tpe 'init_prog 'init ['@list_append; 'string_append]) 
   as init_prog_proof.
 Proof.
   time relcompile.
@@ -47,70 +51,13 @@ Proof.
   time relcompile.
 Qed.
 
-Derive nat_modulo_prog
-  in ltac2:(relcompile_tpe 'nat_modulo_prog 'nat_modulo []) 
-  as nat_modulo_prog_proof.
-Proof.
-  time relcompile.
-  ltac1:(lia).
-Qed.
-
-Derive N_modulo_prog
-  in ltac2:(relcompile_tpe 'N_modulo_prog 'N_modulo []) 
-  as N_modulo_prog_proof.
-Proof.
-  time relcompile.
-  ltac1:(lia).
-Qed.
-
-Theorem N_modulo_bounds: forall n b,
-  (0 <> b)%N ->
-  (N_modulo n b < b)%N.
-Proof.
-  intros; unfold N_modulo.
-  destruct (N.to_nat b); try ltac1:(lia).
-  unfold dlet.
-  rewrite <- N.Div0.mod_eq.
-  destruct b eqn:?; try ltac1:(lia).
-  eapply N.mod_upper_bound.
-  ltac1:(lia).
-Qed.
-
-Derive name2str_prog
+(* Derive name2str_prog
   in ltac2:(relcompile_tpe 'name2str_prog 'name2str ['N_modulo]) 
   as name2str_prog_proof.
 Proof.
   time relcompile.
   subst; eapply N_modulo_bounds; ltac1:(lia).
-Qed.
-
-Derive list_append_prog
-  in ltac2:(relcompile_tpe 'list_append_prog '@list_append []) 
-  as list_append_prog_proof.
-Proof.
-  time relcompile.
-Qed.
-
-Derive list_length_prog
-  in ltac2:(relcompile_tpe 'list_length_prog '@list_length []) 
-  as list_length_prog_proof.
-Proof.
-  time relcompile.
-Qed.
-
-Derive flatten_prog
-  in ltac2:(relcompile_tpe 'flatten_prog '@flatten ['@list_append]) 
-  as flatten_prog_proof.
-Proof.
-  time relcompile.
-Qed.
-
-Derive app_list_length_prog
-  in ltac2:(relcompile_tpe 'app_list_length_prog '@app_list_length ['@list_length]) 
-  as app_list_length_prog_proof.
-Proof.
-  time relcompile.
-Qed.
+Qed. *)
 
 Derive give_up_prog 
   in ltac2:(relcompile_tpe 'give_up_prog 'give_up []) 
@@ -133,8 +80,6 @@ Proof.
   time relcompile.
 Qed.
 
-(* Derivations with dependencies *)
-
 Derive even_len_prog 
   in ltac2:(relcompile_tpe 'even_len_prog '@even_len []) 
   as even_len_prog_proof.
@@ -150,7 +95,7 @@ Proof.
 Qed.
 
 Derive index_of_prog 
-  in ltac2:(relcompile_tpe 'index_of_prog 'index_of ['index_of]) 
+  in ltac2:(relcompile_tpe 'index_of_prog 'index_of []) 
   as index_of_prog_proof.
 Proof.
   time relcompile.
@@ -291,7 +236,7 @@ Proof.
 Qed.
 
 Derive c_store_prog 
-  in ltac2:(relcompile_tpe 'c_store_prog 'c_store []) 
+  in ltac2:(relcompile_tpe 'c_store_prog 'c_store ['@list_append])
   as c_store_prog_proof.
 Proof.
   time relcompile.
@@ -319,7 +264,7 @@ Proof.
 Qed.
 
 Derive c_test_jump_prog 
-  in ltac2:(relcompile_tpe 'c_test_jump_prog 'c_test_jump ['c_exp; 'c_cmp; '@app_list_length]) 
+  in ltac2:(relcompile_tpe 'c_test_jump_prog 'c_test_jump ['c_exp; 'c_cmp; '@app_list_length; '@list_append]) 
   as c_test_jump_prog_proof.
 Proof.
   time relcompile.
@@ -393,7 +338,7 @@ Proof.
 Qed.
 
 Derive c_fundefs_prog 
-  in ltac2:(relcompile_tpe 'c_fundefs_prog 'c_fundefs ['c_fundef; 'name2str; 'name_of_func]) 
+  in ltac2:(relcompile_tpe 'c_fundefs_prog 'c_fundefs ['c_fundef; 'name_of_func]) 
   as c_fundefs_prog_proof.
 Proof.
   time relcompile.
@@ -406,26 +351,281 @@ Proof.
   time relcompile.
 Qed.
 
-(* Derive codegen_program_prog
-  in (
-    ∀ functions : list FunSyntax.func,
-    codegen_program_prog = 
-    ∀ body : FunSyntax.exp,
-      codegen_prog = FunSyntax.Defun (name_enc "codegen") ([name_enc "prog"] : list N) body →
-      ∀ s : state,
-      (∀ (ds : list func) (l : nat) (fs : f_lookup),
-      eval_app (name_enc "c_fundefs") [encode ds; encode l; encode fs] s
-      (encode (c_fundefs ds l fs), s)) →
-      (∀ (fs : f_lookup) (n : N),
-        eval_app (name_enc "lookup") [encode fs; encode n] s (encode (lookup fs n), s))
-      (∀ k : nat, eval_app (name_enc "init") [encode k] s (encode (init k), s)) →
-      (∀ p : prog, eval_app (name_enc "get_funcs") [encode p] s (encode (get_funcs p), s)) →
-      (∀ (A : Type) (Refinable_inst : Refinable A) (xs : app_list A),
-        eval_app (name_enc "app_list_length") [encode xs] s
-        (encode (app_list_length xs), s)) →
-      (∀ (A : Type) (Refinable_inst : Refinable A) (xs : app_list A),
-        eval_app (name_enc "flatten") [encode xs] s (encode (flatten xs), s)) →
-      lookup_fun (name_enc "codegen") (funs s) = Some ([name_enc "prog"] : list N, body) →
-      ∀ prog : ImpSyntax.prog,
-        eval_app (name_enc "codegen") [encode prog] s (encode (codegen prog), s)
-  ) as codegen_program_prog_proof. *)
+Definition ImpToASMCodegen_funs := [
+  init_prog;                    (* 0 *)
+  c_assign_prog;               (* 1 *)
+  list_append_prog;            (* 2 *)
+  list_length_prog;            (* 3 *)
+  flatten_prog;                (* 4 *)
+  app_list_length_prog;        (* 5 *)
+  give_up_prog;                (* 6 *)
+  abortLoc_prog;               (* 7 *)
+  c_const_prog;                (* 8 *)
+  even_len_prog;               (* 9 *)
+  odd_len_prog;                (* 10 *)
+  index_of_prog;               (* 11 *)
+  index_of_opt_prog;           (* 12 *)
+  c_var_prog;                  (* 13 *)
+  all_binders_prog;            (* 14 *)
+  names_contain_prog;          (* 15 *)
+  names_unique_prog;           (* 16 *)
+  unique_binders_prog;         (* 17 *)
+  make_vs_from_binders_prog;   (* 18 *)
+  filter_name_prog;            (* 19 *)
+  remove_names_prog;           (* 20 *)
+  call_v_stack_prog;           (* 21 *)
+  c_pushes_vs_prog;            (* 22 *)
+  c_declare_binders_prog;      (* 23 *)
+  c_add_prog;                  (* 24 *)
+  c_sub_prog;                  (* 25 *)
+  c_div_prog;                  (* 26 *)
+  c_alloc_prog;                (* 27 *)
+  c_read_prog;                 (* 28 *)
+  c_write_prog;                (* 29 *)
+  c_load_prog;                 (* 30 *)
+  c_store_prog;                (* 31 *)
+  c_exp_prog;                  (* 32 *)
+  c_exps_prog;                 (* 33 *)
+  c_cmp_prog;                  (* 34 *)
+  c_test_jump_prog;            (* 35 *)
+  lookup_prog;                 (* 36 *)
+  make_ret_prog;               (* 37 *)
+  c_pops_prog;                 (* 38 *)
+  c_pushes_prog;               (* 39 *)
+  c_call_prog;                 (* 40 *)
+  c_cmd_prog;                  (* 41 *)
+  c_fundef_prog;               (* 42 *)
+  get_funcs_prog;              (* 43 *)
+  name_of_func_prog;           (* 44 *)
+  c_fundefs_prog;              (* 45 *)
+  codegen_prog                 (* 46 *)
+].
+
+From impboot Require Import automation.ltac2.Messages.
+
+Ltac2 assert_lookup_fun (prog: constr) :=
+  let h := Fresh.in_goal (Option.get (Ident.of_string "Hlookup_fun_s")) in
+  assert (match $prog with
+  | FunSyntax.Defun fname args fn =>
+      lookup_fun fname (funs &s) = Some (args, fn)
+  end) as $h; try (simpl in $h).
+
+Ltac2 assert_eval_app (fname: constr) :=
+  let tpe := gen_eval_app fname () in
+  assert ($tpe).
+
+Ltac2 assert_eval_app_proof (prf: constr) (list_constr: constr) (n: int) :=
+  eapply $prf; eauto; try (reflexivity);
+  try (eapply $list_constr; do n (eapply in_cons); eapply in_eq).
+
+Ltac2 assert_eval_app_by (fname: constr) (prf: constr) (list_constr_hyp: constr) (n: int) :=
+  let tpe := gen_eval_app fname () in
+  assert ($tpe) by (
+    print_full_goal ();
+    eapply $prf; eauto; try (reflexivity);
+    print_full_goal ();
+    eapply $list_constr_hyp; do n (eapply in_cons); eapply in_eq
+  ).
+
+Ltac2 int_to_constr_nat (n: int) : constr :=
+  let rec go n acc :=
+    if Int.equal n 0 then acc
+    else go (Int.sub n 1) (constr:(S $acc))
+  in
+  go n (constr:(O)).
+
+Require Import Ltac2.RedFlags.
+Require Import Ltac2.Printf.
+From Ltac2 Require Import Std.
+
+From coqutil Require Import Tactics.reference_to_string.
+
+Ltac2 loop_assert_eval_app_in_list (list_constr: constr) (size: int) :=
+  let rec go n :=
+    if Int.equal n size then ()
+    else (
+      let n_constr := int_to_constr_nat n in
+      let prog := constr:(nth $n_constr $list_constr (FunSyntax.Defun (name_enc "dummy") [] (FunSyntax.Const 0))) in
+      let prog := Std.eval_simpl all None prog in
+      (* remove prog from the prog name *)
+      let prog_ref := reference_of_constr prog in
+      let prog_ref_str := Option.get (reference_to_string prog_ref) in
+      let prf_str := String.app prog_ref_str "_proof" in
+      let prf := Option.get (Ident.of_string prf_str) in
+      let prf_constr := Env.instantiate (VarRef prf) in
+      let fname_str := String.sub prog_ref_str 0 (Int.sub (String.length prog_ref_str) (String.length "_prog")) in
+      let fname := Option.get (Ident.of_string fname_str) in
+      let fname_constr := Env.instantiate (VarRef fname) in
+      assert_eval_app_by fname_constr prf_constr list_constr n;
+      go (Int.add n 1)
+    )
+  in
+  go 0.
+
+Theorem codegen_thm:
+  ∀ (s: state) (p: prog),
+    (∀ fname args fn,
+      In (FunSyntax.Defun fname args fn) (CompilerUtils_funs) →
+      lookup_fun fname (funs s) = Some (args, fn)) ->
+    (∀ fname args fn,
+      In (FunSyntax.Defun fname args fn) (ImpToASMCodegen_funs) →
+      lookup_fun fname (funs s) = Some (args, fn)) ->
+    eval_app (name_enc "codegen") [encode p] s ((encode (codegen p)), s).
+Proof.
+  intros * Hlookup_fun_utils Hlookup_fun.
+  assert_eval_app_by 'mul_nat 'mul_nat_prog_proof 'Hlookup_fun_utils 0.
+  assert_eval_app_by 'mul_N_f 'mul_N_f_prog_proof 'Hlookup_fun_utils 1.
+  assert_eval_app_by 'mul_N 'mul_N_prog_proof 'Hlookup_fun_utils 2.
+  assert_eval_app_by 'nat_modulo 'nat_modulo_prog_proof 'Hlookup_fun_utils 3.
+  assert_eval_app_by 'N_modulo 'N_modulo_prog_proof 'Hlookup_fun_utils 4.
+  assert_eval_app_by 'num2str_f 'num2str_f_prog_proof 'Hlookup_fun_utils 5.
+  assert_eval_app_by 'num2str 'num2str_prog_proof 'Hlookup_fun_utils 6.
+  assert_eval_app_by 'N2str_f 'N2str_f_prog_proof 'Hlookup_fun_utils 7.
+  assert_eval_app_by 'N2str 'N2str_prog_proof 'Hlookup_fun_utils 8.
+  assert_eval_app_by 'list_length 'list_length_prog_proof 'Hlookup_fun_utils 9.
+  assert_eval_app_by 'list_append 'list_append_prog_proof 'Hlookup_fun_utils 10.
+  assert_eval_app_by 'flatten 'flatten_prog_proof 'Hlookup_fun_utils 11.
+  assert_eval_app_by 'app_list_length 'app_list_length_prog_proof 'Hlookup_fun_utils 12.
+  assert_eval_app_by 'string_append 'string_append_prog_proof 'Hlookup_fun_utils 13.
+  assert_eval_app_by 'mul_nat 'mul_nat_prog_proof 'Hlookup_fun_utils 14.
+
+
+  
+  loop_assert_eval_app_in_list (constr:(CompilerUtils_funs)) 17.
+  assert_eval_app '@list_length.
+  1: {
+    eapply list_length_prog_proof; eauto; try reflexivity.
+    1: eapply Hlookup_fun; do 53 (eapply in_cons); eapply in_eq.
+  }
+  assert_eval_app '@list_append.
+  1: {
+    eapply list_append_prog_proof; eauto; try reflexivity.
+    1: eapply Hlookup_fun; do 54 (eapply in_cons); eapply in_eq.
+  }
+  assert_eval_app '@app_list_length.
+  1: {
+    eapply app_list_length_prog_proof; eauto; try reflexivity.
+    1: eapply Hlookup_fun; do 56 (eapply in_cons); eapply in_eq.
+  }
+  assert_eval_app 'call_v_stack.
+  1: {
+    eapply call_v_stack_prog_proof; eauto; try reflexivity.
+    1: eapply Hlookup_fun; do 21 (eapply in_cons); eapply in_eq.
+  }
+  assert_eval_app '@even_len.
+  1: {
+    eapply even_len_prog_proof; eauto; try reflexivity.
+    1: eapply Hlookup_fun; do 9 (eapply in_cons); eapply in_eq.
+  }
+  assert_eval_app 'c_pushes.
+  1: {
+    eapply c_pushes_prog_proof; eauto; try reflexivity.
+    2: eapply Hlookup_fun; do 39 (eapply in_cons); eapply in_eq.
+    eapply c_pushes_vs_prog_proof; eauto; try reflexivity.
+    eapply Hlookup_fun; do 22 (eapply in_cons); eapply in_eq.
+  }
+  assert_eval_app 'unique_binders.
+  1: {
+    eapply unique_binders_prog_proof; eauto; try reflexivity.  
+    3: eapply Hlookup_fun; do 17 (eapply in_cons); eapply in_eq.
+    1: eapply all_binders_prog_proof; eauto; try reflexivity.
+    1: eapply Hlookup_fun; do 14 (eapply in_cons); eapply in_eq.
+    1: eapply names_unique_prog_proof; eauto; try reflexivity.
+    2: eapply Hlookup_fun; do 16 (eapply in_cons); eapply in_eq.
+    eapply names_contain_prog_proof; eauto; try reflexivity.
+    eapply Hlookup_fun; do 15 (eapply in_cons); eapply in_eq.
+  }
+  assert_eval_app 'string_append.
+  1: {
+    eapply string_append_prog_proof; eauto; try reflexivity.
+    eapply Hlookup_fun; do 60 (eapply in_cons); eapply in_eq.
+  }
+  eapply codegen_prog_proof; eauto; try reflexivity.
+  6: eapply Hlookup_fun; do 46 (eapply in_cons); eapply in_eq.
+  5: eapply flatten_prog_proof; eauto; try reflexivity.
+  5: eapply Hlookup_fun; do 55 (eapply in_cons); eapply in_eq.
+  1: eapply c_fundefs_prog_proof; eauto; try reflexivity.
+  3: eapply Hlookup_fun; do 45 (eapply in_cons); eapply in_eq.
+  1: eapply c_fundef_prog_proof; eauto; try reflexivity.
+  4: eapply Hlookup_fun; do 42 (eapply in_cons); eapply in_eq.
+  7: eapply get_funcs_prog_proof; eauto; try reflexivity.
+  7: eapply Hlookup_fun; do 43 (eapply in_cons); eapply in_eq.
+  6: eapply init_prog_proof; eauto; try reflexivity.
+  6: eapply Hlookup_fun; do 0 (eapply in_cons); eapply in_eq.
+  5: eapply lookup_prog_proof; eauto; try reflexivity.
+  5: eapply Hlookup_fun; do 36 (eapply in_cons); eapply in_eq.
+  4: eapply name_of_func_prog_proof; eauto; try reflexivity.
+  4: eapply Hlookup_fun; do 44 (eapply in_cons); eapply in_eq.
+  1: eapply make_vs_from_binders_prog_proof; eauto; try reflexivity.
+  1: eapply Hlookup_fun; do 18 (eapply in_cons); eapply in_eq.
+  2: eapply c_declare_binders_prog_proof; eauto; try reflexivity.
+  5: eapply Hlookup_fun; do 23 (eapply in_cons); eapply in_eq.
+  4: eapply c_pushes_vs_prog_proof; eauto; try reflexivity.
+  4: eapply Hlookup_fun; do 22 (eapply in_cons); eapply in_eq.
+  3: eapply make_vs_from_binders_prog_proof; eauto; try reflexivity.
+  3: eapply Hlookup_fun; do 18 (eapply in_cons); eapply in_eq.
+  2: eapply remove_names_prog_proof; eauto; try reflexivity.
+  3: eapply Hlookup_fun; do 20 (eapply in_cons); eapply in_eq.
+  2: eapply filter_name_prog_proof; eauto; try reflexivity.
+  2: eapply Hlookup_fun; do 19 (eapply in_cons); eapply in_eq.
+  assert_eval_app 'c_exp.
+  1: {
+    eapply c_exp_prog_proof; eauto; try reflexivity.
+    7: eapply Hlookup_fun; do 32 (eapply in_cons); eapply in_eq.
+    1: eapply c_var_prog_proof; eauto; try reflexivity.
+    2: eapply Hlookup_fun; do 13 (eapply in_cons); eapply in_eq.
+    1: eapply index_of_prog_proof; eauto; try reflexivity.
+    1: eapply Hlookup_fun; do 11 (eapply in_cons); eapply in_eq.
+    1: eapply c_const_prog_proof; eauto; try reflexivity.
+    1: eapply Hlookup_fun; do 8 (eapply in_cons); eapply in_eq.
+    1: eapply c_add_prog_proof; eauto; try reflexivity.
+    1: eapply Hlookup_fun; do 24 (eapply in_cons); eapply in_eq.
+    1: eapply c_sub_prog_proof; eauto; try reflexivity.
+    1: eapply Hlookup_fun; do 25 (eapply in_cons); eapply in_eq.
+    1: eapply c_div_prog_proof; eauto; try reflexivity.
+    1: eapply Hlookup_fun; do 26 (eapply in_cons); eapply in_eq.
+    1: eapply c_load_prog_proof; eauto; try reflexivity.
+    1: eapply Hlookup_fun; do 30 (eapply in_cons); eapply in_eq.
+  }
+  assert_eval_app 'c_assign.
+  1: {
+    eapply c_assign_prog_proof; eauto; try reflexivity.
+    2: eapply Hlookup_fun; do 1 (eapply in_cons); eapply in_eq.
+    eapply index_of_prog_proof; eauto; try reflexivity.
+    eapply Hlookup_fun; do 11 (eapply in_cons); eapply in_eq.
+  }
+  eapply c_cmd_prog_proof; eauto; try reflexivity.
+  13: eapply Hlookup_fun; do 41 (eapply in_cons); eapply in_eq.
+  1: eapply c_store_prog_proof; eauto; try reflexivity.
+  1: eapply Hlookup_fun; do 31 (eapply in_cons); eapply in_eq.
+  1: eapply c_test_jump_prog_proof; eauto; try reflexivity.
+  2: eapply Hlookup_fun; do 35 (eapply in_cons); eapply in_eq.
+  1: eapply c_cmp_prog_proof; eauto; try reflexivity.
+  1: eapply Hlookup_fun; do 34 (eapply in_cons); eapply in_eq.
+  1: eapply c_exps_prog_proof; eauto; try reflexivity.
+  1: eapply Hlookup_fun; do 33 (eapply in_cons); eapply in_eq.
+  1: eapply c_call_prog_proof; eauto; try reflexivity.
+  2: eapply Hlookup_fun; do 40 (eapply in_cons); eapply in_eq.
+  1: eapply c_pops_prog_proof; eauto; try reflexivity.
+  2: eapply Hlookup_fun; do 38 (eapply in_cons); eapply in_eq.
+  1: eapply give_up_prog_proof; eauto; try reflexivity.
+  1: eapply Hlookup_fun; do 6 (eapply in_cons); eapply in_eq.
+  1: eapply c_var_prog_proof; eauto; try reflexivity.
+  2: eapply Hlookup_fun; do 13 (eapply in_cons); eapply in_eq.
+  1: eapply index_of_prog_proof; eauto; try reflexivity.
+  1: eapply Hlookup_fun; do 11 (eapply in_cons); eapply in_eq.
+  1: eapply make_ret_prog_proof; eauto; try reflexivity.
+  1: eapply Hlookup_fun; do 37 (eapply in_cons); eapply in_eq.
+  1: eapply c_alloc_prog_proof; eauto; try reflexivity.
+  1: eapply Hlookup_fun; do 27 (eapply in_cons); eapply in_eq.
+  1: eapply c_read_prog_proof; eauto; try reflexivity.
+  1: eapply Hlookup_fun; do 28 (eapply in_cons); eapply in_eq.
+  1: eapply c_write_prog_proof; eauto; try reflexivity.
+  1: eapply Hlookup_fun; do 29 (eapply in_cons); eapply in_eq.
+  1: eapply abortLoc_prog_proof; eauto; try reflexivity.
+  1: eapply Hlookup_fun; do 7 (eapply in_cons); eapply in_eq.
+  1: eapply lookup_prog_proof; eauto; try reflexivity.
+  1: eapply Hlookup_fun; do 36 (eapply in_cons); eapply in_eq.
+  eapply odd_len_prog_proof; eauto; try reflexivity.
+  eapply Hlookup_fun; do 10 (eapply in_cons); eapply in_eq.
+Qed.
