coq/theories/derivations/ParserDerivations.v
@@ -7,7 +7,7 @@ Require Import impboot.utils.AppList.
 Require Import impboot.parsing.Parser.
 Require Import impboot.imp2asm.ImpToASMCodegen.
 From impboot Require Import automation.Ltac2Utils.
-From impboot Require Import commons.PrintingUtils.
+From impboot Require Import commons.CompilerUtils.
 From impboot Require Import functional.FunValues.
 From impboot Require Import functional.FunSemantics.
 Require Import impboot.automation.RelCompiler.
@@ -20,10 +20,12 @@ From Stdlib Require Import derive.Derive.
 From Stdlib Require Import Lia.
 From Ltac2 Require Import Ltac2.
 
+From impboot Require Import derivations.CompilerUtilsDerivations.
+
 (* lexing *)
 
-(* Derive read_num_prog
-  in ltac2:(relcompile_tpe 'read_num_prog 'read_num [])
+Derive read_num_prog
+  in ltac2:(relcompile_tpe 'read_num_prog 'read_num ['mul_N])
   as read_num_prog_proof.
 Proof.
   time relcompile.
@@ -62,7 +64,7 @@ Derive lexer_prog
   as lexer_prog_proof.
 Proof.
   time relcompile.
-Qed. *)
+Qed.
 
 (* FunValues *)
 
@@ -80,6 +82,8 @@ Proof.
   time relcompile.
 Qed.
 
+Theorem vlist_equation: ltac2:(unfold_fix_type '@vlist).
+Proof. unfold_fix_proof '@vlist. Qed.
 Derive vlist_prog
   in ltac2:(relcompile_tpe 'vlist_prog 'vlist ['vcons])
   as vlist_prog_proof.
@@ -114,6 +118,34 @@ Qed.
 Derive vel0_prog
   in ltac2:(relcompile_tpe 'vel0_prog 'vel0 ['vhead])
   as vel0_prog_proof.
+Proof.
+  time relcompile.
+Qed.
+
+Derive vel1_prog
+  in ltac2:(relcompile_tpe 'vel1_prog 'vel1 ['vhead; 'vtail])
+  as vel1_prog_proof.
+Proof.
+  time relcompile.
+Qed.
+
+Derive vel2_prog
+  in ltac2:(relcompile_tpe 'vel2_prog 'vel2 ['vel1; 'vtail])
+  as vel2_prog_proof.
+Proof.
+  time relcompile.
+Qed.
+
+Derive vel3_prog
+  in ltac2:(relcompile_tpe 'vel3_prog 'vel3 ['vel2; 'vtail])
+  as vel3_prog_proof.
+Proof.
+  time relcompile.
+Qed.
+
+Derive vtail_prog
+  in ltac2:(relcompile_tpe 'vtail_prog 'vtail [])
+  as vtail_prog_proof.
 Proof.
   time relcompile.
 Qed.
@@ -162,7 +194,8 @@ Derive num2exp_prog
   as num2exp_prog_proof.
 Proof.
   time relcompile.
-  subst; eapply N_modulo_lt; ltac1:(lia).
+  subst; specialize N_modulo_lt with (n := n) (m := (2 ^ 64 - 1)%N) as Hlt.
+  ltac1:(lia).
 Qed.
 
 Derive v2exp_prog
@@ -170,7 +203,8 @@ Derive v2exp_prog
   as v2exp_prog_proof.
 Proof.
   time relcompile.
-  subst; eapply N_modulo_lt; ltac1:(lia).
+  subst; specialize N_modulo_lt with (n := (vgetNum v0_3)) (m := (2 ^ 64 - 1)%N) as Hlt.
+  ltac1:(lia).
 Qed.
 
 Derive vs2exps_prog
@@ -243,4 +277,180 @@ Derive str2imp_prog
   as str2imp_prog_proof.
 Proof.
   time relcompile.
+Qed.
+
+Definition ParserDerivations_funs := [
+  read_num_prog;
+  end_line_prog;
+  q_from_nat_prog;
+  lex_prog;
+  lexer_i_prog;
+  lexer_prog;
+  vcons_prog;
+  vhead_prog;
+  vlist_prog;
+  vis_upper_f_prog;
+  vis_upper_prog;
+  vgetNum_prog;
+  vel0_prog;
+  visNum_prog;
+  visPair_prog;
+  quote_prog;
+  parse_prog;
+  v2list_prog;
+  num2exp_prog;
+  v2exp_prog;
+  vs2exps_prog;
+  v2cmp_prog;
+  v2test_prog;
+  v2cmd_prog;
+  vs2args_prog;
+  v2func_prog;
+  v2funcs_prog;
+  vs2prog_prog;
+  parser_prog;
+  str2imp_prog;
+  vel1_prog;
+  vel2_prog;
+  vel3_prog;
+  vtail_prog
+].
+
+Ltac2 assert_lookup_fun (prog: constr) :=
+  let h := Fresh.in_goal (Option.get (Ident.of_string "Hlookup_fun_s")) in
+  assert (match $prog with
+  | FunSyntax.Defun fname args fn =>
+      lookup_fun fname (funs &s) = Some (args, fn)
+  end) as $h; try (simpl in $h).
+
+Theorem str2imp_thm:
+  ∀ (s: state) (inp: list ascii),
+    (∀ fname args fn,
+      In (FunSyntax.Defun fname args fn) (ParserDerivations_funs ++ CompilerUtils_funs) →
+      lookup_fun fname (funs s) = Some (args, fn)) ->
+    eval_app (name_enc "str2imp") [encode inp] s ((encode (str2imp inp)), s).
+Proof.
+  Opaque encode.
+  intros * Hlookup_fun.
+  assert_lookup_fun 'vel1_prog; simpl.
+  1: eapply Hlookup_fun; do 30 (eapply in_cons); eapply in_eq.
+  assert_lookup_fun 'vel2_prog; simpl.
+  1: eapply Hlookup_fun; do 31 (eapply in_cons); eapply in_eq.
+  assert_lookup_fun 'vel3_prog; simpl.
+  1: eapply Hlookup_fun; do 32 (eapply in_cons); eapply in_eq.
+  assert_lookup_fun 'list_length_prog; simpl.
+  1: eapply Hlookup_fun; do 40 (eapply in_cons); eapply in_eq.
+  assert_lookup_fun 'vhead_prog; simpl.
+  1: eapply Hlookup_fun; do 7 (eapply in_cons); eapply in_eq.
+  assert_lookup_fun 'vtail_prog; simpl.
+  1: eapply Hlookup_fun; do 33 (eapply in_cons); eapply in_eq.
+  assert_lookup_fun 'vgetNum_prog; simpl.
+  1: eapply Hlookup_fun; do 11 (eapply in_cons); eapply in_eq.
+  assert_lookup_fun 'vhead_prog; simpl.
+  1: eapply Hlookup_fun; do 7 (eapply in_cons); eapply in_eq.
+  assert_lookup_fun 'vel0_prog; simpl.
+  1: eapply Hlookup_fun; do 12 (eapply in_cons); eapply in_eq.
+  assert_lookup_fun 'N_modulo_prog; simpl.
+  1: eapply Hlookup_fun; do 35 (eapply in_cons); eapply in_eq.
+  assert_lookup_fun 'mul_N_prog; simpl.
+  1: eapply Hlookup_fun; do 46 (eapply in_cons); eapply in_eq.
+  assert_lookup_fun 'mul_N_f_prog; simpl.
+  1: eapply Hlookup_fun; do 45 (eapply in_cons); eapply in_eq.
+  eapply str2imp_prog_proof; eauto; try reflexivity.
+  3: eapply Hlookup_fun; do 29 (eapply in_cons); eapply in_eq.
+  1: {
+    eapply lexer_prog_proof; eauto; try reflexivity.
+    2: eapply Hlookup_fun; do 5 (eapply in_cons); eapply in_eq.
+    eapply lexer_i_prog_proof; eauto; try reflexivity.
+    3: eapply Hlookup_fun; do 4 (eapply in_cons); eapply in_eq.
+    2: eapply list_length_prog_proof; eauto; try reflexivity.
+    eapply lex_prog_proof; eauto; try reflexivity.
+    5: eapply Hlookup_fun; do 3 (eapply in_cons); eapply in_eq.
+    1: eapply end_line_prog_proof; eauto; try reflexivity.
+    1: eapply Hlookup_fun; do 1 (eapply in_cons); eapply in_eq.
+    1: eapply read_num_prog_proof; eauto; try reflexivity.
+    2: eapply Hlookup_fun; do 0 (eapply in_cons); eapply in_eq.
+    1: eapply mul_N_prog_proof; eauto; try reflexivity.
+    1: eapply mul_N_f_prog_proof; eauto; try reflexivity.
+    1: eapply q_from_nat_prog_proof; eauto; try reflexivity.
+    1: eapply Hlookup_fun; do 2 (eapply in_cons); eapply in_eq.
+    eapply list_length_prog_proof; eauto; try reflexivity.
+  }
+  eapply parser_prog_proof; eauto; try reflexivity.
+  4: eapply Hlookup_fun; do 28 (eapply in_cons); eapply in_eq.
+  1: {
+    eapply parse_prog_proof; eauto; try reflexivity.
+    3: eapply Hlookup_fun; do 16 (eapply in_cons); eapply in_eq.
+    1: eapply vhead_prog_proof; eauto; try reflexivity.
+    eapply quote_prog_proof; eauto; try reflexivity.
+    2: eapply Hlookup_fun; do 15 (eapply in_cons); eapply in_eq.
+    eapply vlist_prog_proof; eauto; try reflexivity.
+    2: eapply Hlookup_fun; do 8 (eapply in_cons); eapply in_eq.
+    eapply vcons_prog_proof; eauto; try reflexivity.
+    1: eapply Hlookup_fun; do 6 (eapply in_cons); eapply in_eq.
+  }
+  1: eapply v2list_prog_proof; eauto; try reflexivity.
+  1: eapply Hlookup_fun; do 17 (eapply in_cons); eapply in_eq.
+  eapply vs2prog_prog_proof; eauto; try reflexivity.
+  2: eapply Hlookup_fun; do 27 (eapply in_cons); eapply in_eq.
+  eapply v2funcs_prog_proof; eauto; try reflexivity.
+  2: eapply Hlookup_fun; do 26 (eapply in_cons); eapply in_eq.
+  assert (∀ v : Value, eval_app (name_enc "v2exp") [encode v] s (encode (v2exp v), s)).
+  1: eapply v2exp_prog_proof; eauto; try reflexivity.
+  5: eapply Hlookup_fun; do 19 (eapply in_cons); eapply in_eq.
+  1: eapply vgetNum_prog_proof; eauto; try reflexivity.
+  1: eapply vel0_prog_proof; eauto; try reflexivity.
+  1: eapply vhead_prog_proof; eauto; try reflexivity.  
+  1: eapply num2exp_prog_proof; eauto; try reflexivity.
+  3: eapply Hlookup_fun; do 18 (eapply in_cons); eapply in_eq.
+  1: eapply vis_upper_prog_proof; eauto; try reflexivity.
+  2: eapply Hlookup_fun; do 10 (eapply in_cons); eapply in_eq.
+  1: eapply vis_upper_f_prog_proof; eauto; try reflexivity.
+  1: eapply Hlookup_fun; do 9 (eapply in_cons); eapply in_eq.
+  1: eapply N_modulo_prog_proof; eauto; try reflexivity.
+  2: eapply N_modulo_prog_proof; eauto; try reflexivity.
+  1: eapply mul_N_prog_proof; eauto; try reflexivity.
+  1: eapply mul_N_f_prog_proof; eauto; try reflexivity.
+  1: eapply mul_N_prog_proof; eauto; try reflexivity.
+  1: eapply mul_N_f_prog_proof; eauto; try reflexivity.
+  eapply v2func_prog_proof; eauto; try reflexivity.
+  8: eapply Hlookup_fun; do 25 (eapply in_cons); eapply in_eq.
+  1: eapply vel1_prog_proof; eauto; try reflexivity.
+  1: eapply vhead_prog_proof; eauto; try reflexivity.
+  1: eapply vtail_prog_proof; eauto; try reflexivity.
+  1: eapply vel2_prog_proof; eauto; try reflexivity.
+  1: eapply vel1_prog_proof; eauto; try reflexivity.
+  1: eapply vhead_prog_proof; eauto; try reflexivity.
+  1: eapply vtail_prog_proof; eauto; try reflexivity.
+  1: eapply vtail_prog_proof; eauto; try reflexivity.
+  1: eapply vel3_prog_proof; eauto; try reflexivity.
+  1: eapply vel2_prog_proof; eauto; try reflexivity.
+  1: eapply vel1_prog_proof; eauto; try reflexivity.
+  1: eapply vhead_prog_proof; eauto; try reflexivity.
+  1: eapply vtail_prog_proof; eauto; try reflexivity.
+  1: eapply vtail_prog_proof; eauto; try reflexivity.
+  1: eapply vtail_prog_proof; eauto; try reflexivity.
+  1: eapply vgetNum_prog_proof; eauto; try reflexivity.
+  1: eapply v2list_prog_proof; eauto; try reflexivity.
+  1: eapply Hlookup_fun; do 17 (eapply in_cons); eapply in_eq.
+  1: eapply vs2args_prog_proof; eauto; try reflexivity.
+  2: eapply Hlookup_fun; do 24 (eapply in_cons); eapply in_eq.
+  1: eapply vgetNum_prog_proof; eauto; try reflexivity.
+  1: eapply v2cmd_prog_proof; eauto; try reflexivity.
+  7: eapply Hlookup_fun; do 23 (eapply in_cons); eapply in_eq.
+  1: eapply vgetNum_prog_proof; eauto; try reflexivity.
+  2: eapply v2list_prog_proof; eauto; try reflexivity.
+  2: eapply Hlookup_fun; do 17 (eapply in_cons); eapply in_eq.
+  4: eapply visPair_prog_proof; eauto; try reflexivity.
+  4: eapply Hlookup_fun; do 14 (eapply in_cons); eapply in_eq.
+  3: eapply visNum_prog_proof; eauto; try reflexivity.
+  3: eapply Hlookup_fun; do 13 (eapply in_cons); eapply in_eq.
+  2: eapply vs2exps_prog_proof; eauto; try reflexivity.
+  2: eapply Hlookup_fun; do 20 (eapply in_cons); eapply in_eq.
+  1: eapply v2test_prog_proof; eauto; try reflexivity.
+  3: eapply Hlookup_fun; do 22 (eapply in_cons); eapply in_eq.
+  1: eapply vgetNum_prog_proof; eauto; try reflexivity.
+  1: eapply v2cmp_prog_proof; eauto; try reflexivity.
+  2: eapply Hlookup_fun; do 21 (eapply in_cons); eapply in_eq.
+  eapply vgetNum_prog_proof; eauto; try reflexivity.
 Qed.
