coq/theories/imp2asm/Compiler.v
@@ -5,7 +5,7 @@ Require Import impboot.imperative.ImpSyntax.
 Require Import impboot.parsing.Parser.
 Require Import impboot.assembly.ASMToString.
 
-Definition compiler (inp: string): string :=
+Definition compiler (inp: list ascii): string :=
   let/d p := str2imp inp in
   let/d asm := codegen p in
   let/d str := asm2str asm in
