coq/theories/imp2asm/ImpToASMCodegen.v
@@ -2,11 +2,13 @@ From impboot Require Import utils.Core.
 Require Import impboot.assembly.ASMSyntax.
 Require Import impboot.imperative.ImpSyntax.
 Require Import impboot.utils.AppList.
-Require Import impboot.commons.PrintingUtils.
+Require Import impboot.commons.CompilerUtils.
 Require Import coqutil.Word.Interface.
 Require Import ZArith.
 Require Import FunInd.
 Require Import Ascii.
+
+Require Import impboot.imperative.Printing.
 
 Require Import impboot.automation.ltac2.UnfoldFix.
 Require Import Ltac2.Ltac2.
@@ -21,89 +23,115 @@ Notation f_lookup := (list (name * nat)).
 
 (* Generates the initialization code for execution *)
 Definition init (k: nat): asm :=
-  [
-    (*  0 *) ASMSyntax.Const RAX (word.of_Z (Z.of_nat 0));
-    (*  1 *) ASMSyntax.Const R12 (word.of_Z (Z.of_nat 16));
-    (*  2 *) ASMSyntax.Const R13 (word.of_Z (Z.of_N (2^63 - 1)));
+  let/d rax := RAX in
+  let/d rdi := RDI in
+  let/d r12 := R12 in
+  let/d r13 := R13 in
+  let/d r14 := R14 in
+  let/d r15 := R15 in
+
+  let/d zero_word := word.of_Z (Z.of_nat 0) in
+  let/d instr0 := ASMSyntax.Const rax zero_word in
+  
+  let/d sixteen_word := word.of_Z (Z.of_nat 16) in
+  let/d instr1 := ASMSyntax.Const r12 sixteen_word in
+  
+  let/d max_word := word.of_Z (Z.of_N (2^63 - 1)) in
+  let/d instr2 := ASMSyntax.Const r13 max_word in
+  
+  let/d instr3 := ASMSyntax.Call k in
+  
+  let/d exit_zero_word := word.of_Z (Z.of_nat 0) in
+  let/d instr4 := ASMSyntax.Const rdi exit_zero_word in
+  
+  let/d instr5 := ASMSyntax.Exit in
+  
+  let/d malloc_comment := "malloc" in
+  let/d instr6 := ASMSyntax.Comment malloc_comment in
+  
+  let/d instr7 := ASMSyntax.Mov rax r15 in
+  
+  let/d instr8 := ASMSyntax.Sub rax r14 in
+  
+  let/d cond9 := ASMSyntax.Less r15 r14 in
+  let/d instr9 := ASMSyntax.Jump cond9 15 in
+  
+  let/d cond10 := ASMSyntax.Less rax rdi in
+  let/d instr10 := ASMSyntax.Jump cond10 15 in
+  
+  let/d instr11 := ASMSyntax.Mov rax r14 in
+  
+  let/d instr12 := ASMSyntax.Add r14 rdi in
+  
+  let/d instr13 := ASMSyntax.Ret in
+  
+  let/d exit4_comment := "exit 4" in
+  let/d instr14 := ASMSyntax.Comment exit4_comment in
+  
+  let/d instr15 := ASMSyntax.Push r15 in
+  
+  let/d four_word := word.of_Z (Z.of_nat 4) in
+  let/d instr16 := ASMSyntax.Const rdi four_word in
+  
+  let/d instr17 := ASMSyntax.Exit in
+  
+  let/d exit1_comment := "exit 1" in
+  let/d instr18 := ASMSyntax.Comment exit1_comment in
+  
+  let/d instr19 := ASMSyntax.Push r15 in
+  
+  let/d one_word := word.of_Z (Z.of_nat 1) in
+  let/d instr20 := ASMSyntax.Const rdi one_word in
+  
+  let/d instr21 := ASMSyntax.Exit in
+  
+  let/d list1 := [
+    (*  0 *) instr0;
+    (*  1 *) instr1;
+    (*  2 *) instr2;
     (* jump to main function *)
-    (*  3 *) ASMSyntax.Call k;
+    (*  3 *) instr3
+  ] in
+  let/d list2 := [
     (* return to exit 0 *)
-    (*  4 *) ASMSyntax.Const RDI (word.of_Z (Z.of_nat 0));
-    (*  5 *) ASMSyntax.Exit;
+    (*  4 *) instr4;
+    (*  5 *) instr5;
     (* alloc routine starts here: *)
-    (*  6 *) ASMSyntax.Comment "malloc";
-    (*  7 *) ASMSyntax.Mov RAX R15;
-    (*  8 *) ASMSyntax.Sub RAX R14;
-    (*  9 *) ASMSyntax.Jump (ASMSyntax.Less R15 R14) 15;
-    (* 10 *) ASMSyntax.Jump (ASMSyntax.Less RAX RDI) 15;
-    (* 11 *) ASMSyntax.Mov RAX R14;
-    (* 12 *) ASMSyntax.Add R14 RDI;
-    (* 13 *) ASMSyntax.Ret;
+    (*  6 *) instr6;
+    (*  7 *) instr7
+  ] in
+  let/d list3 := [
+    (*  8 *) instr8;
+    (*  9 *) instr9;
+    (* 10 *) instr10;
+    (* 11 *) instr11
+  ] in
+  let/d list4 := [
+    (* 12 *) instr12;
+    (* 13 *) instr13;
     (* give up: *)
-    (* 14 *) ASMSyntax.Comment "exit 4"; (* Internal error – OOM or compiler limitation *)
-    (* 15 *) ASMSyntax.Push R15; (* align stack *)
-    (* 16 *) ASMSyntax.Const RDI (word.of_Z (Z.of_nat 4));
-    (* 17 *) ASMSyntax.Exit;
+    (* 14 *) instr14; (* Internal error – OOM or compiler limitation *)
+    (* 15 *) instr15 (* align stack *)
+  ] in
+  let/d list5 := [
+    (* 16 *) instr16;
+    (* 17 *) instr17;
     (* abort: *)
-    (* 18 *) ASMSyntax.Comment "exit 1"; (* Internal error – OOM or compiler limitation *)
-    (* 19 *) ASMSyntax.Push R15; (* align stack *)
-    (* 20 *) ASMSyntax.Const RDI (word.of_Z (Z.of_nat 1));
-    (* 21 *) ASMSyntax.Exit
-  ]%string.
+    (* 18 *) instr18; (* Internal error – OOM or compiler limitation *)
+    (* 19 *) instr19 (* align stack *)
+  ] in
+  let/d list6 := [
+    (* 20 *) instr20;
+    (* 21 *) instr21
+  ] in
+  let/d list12 := list_append list1 list2 in
+  let/d list123 := list_append list12 list3 in
+  let/d list1234 := list_append list123 list4 in
+  let/d list12345 := list_append list1234 list5 in
+  let/d result_list := list_append list12345 list6 in
+  result_list.
 
 Definition allocLoc: nat := 7.
-
-(* START boilerplate *)
-
-Fixpoint list_length {A: Type} (l: list A): nat :=
-  match l with
-  | x :: l => 
-    let/d rec := list_length l in
-    let/d res := 1 + rec in 
-    res
-  | [] => 0
-  end.
-Theorem list_length_equation: ltac2:(unfold_fix_type '@list_length).
-Proof. unfold_fix_proof '@list_length. Qed.
-
-Fixpoint list_append {A: Type} (l1 l2: list A): list A :=
-  match l1 with
-  | x :: l1 =>
-    let/d rec := list_append l1 l2 in
-    let/d res := x :: rec in
-    res
-  | [] => l2
-  end.
-Theorem list_append_equation: ltac2:(unfold_fix_type '@list_append).
-Proof. unfold_fix_proof '@list_append. Qed.
-
-Fixpoint flatten {A: Type} (xs: app_list A): list A :=
-  match xs with
-  | List l => l
-  | Append l1 l2 =>
-    let/d flatten_l1 := flatten l1 in
-    let/d flatten_l2 := flatten l2 in
-    let/d res := list_append flatten_l1 flatten_l2 in
-    res
-  end.
-Theorem flatten_equation: ltac2:(unfold_fix_type '@flatten).
-Proof. unfold_fix_proof '@flatten. Qed.
-
-Fixpoint app_list_length {A: Type} (xs: app_list A): nat :=
-  match xs with
-  | List l => 
-    let/d res := list_length l in
-    res
-  | Append l1 l2 =>
-    let/d app_list_length_l1 := app_list_length l1 in
-    let/d app_list_length_l2 := app_list_length l2 in
-    let/d res := app_list_length_l1 + app_list_length_l2 in
-    res
-  end.
-Theorem app_list_length_equation: ltac2:(unfold_fix_type '@app_list_length).
-Proof. unfold_fix_proof '@app_list_length. Qed.
-
-(* END boilerplate *)
 
 Fixpoint even_len {A: Type} (xs: list A): bool :=
   match xs with
@@ -137,8 +165,7 @@ Proof. unfold_fix_proof '@odd_len. Qed.
   b – does the stack need to be aligned
 *)
 Definition give_up (b: bool): nat := 
-  let/d res := if b then 15 else 16 in
-  res.
+  if b then 15 else 16.
 
 Definition abortLoc: nat := 19.
 
@@ -158,17 +185,17 @@ Fixpoint index_of (vs: v_stack) (n: name) (k: nat): nat :=
   | nil => k
   | x :: vs =>
     match x with
-      | None =>
+    | None =>
+      let/d k1 := k + 1 in
+      let/d res := index_of vs n k1 in
+      res
+    | Some v => 
+      if N.eqb v n then
+        k
+      else
         let/d k1 := k + 1 in
         let/d res := index_of vs n k1 in
         res
-      | Some v => 
-        if N.eqb v n then
-          k
-        else
-          let k1 := k + 1 in
-          let/d res := index_of vs n k1 in
-          res
     end
   end.
 Theorem index_of_equation: ltac2:(unfold_fix_type '@index_of).
@@ -220,23 +247,21 @@ Definition c_var (n: name) (l: nat) (vs: v_stack): asm_appl * nat :=
 (* assign variable with name `n`, based on stack *)
 Definition c_assign (n: name) (l: nat) (vs: v_stack): (asm_appl * nat) :=
   let/d k := index_of vs n 0 in
-  match k return (asm_appl * nat) with
-  | 0%nat =>
+  if k =? 0 then
     let/d l1 := l + 1 in
     let/d pop_rdi := ASMSyntax.Pop RDI in
     let/d asm1 := [pop_rdi] in
     let/d asm1 := List asm1 in
     let/d res := (asm1, l1) in
     res
-  | S _ =>
+  else
     let/d l1 := l + 2 in
-    let/d store_rsp_rax := ASMSyntax.Store_RSP RAX k in
+    let/d storersp_rax := ASMSyntax.StoreRSP RAX k in
     let/d pop_rax := ASMSyntax.Pop RAX in
-    let/d asm1 := [store_rsp_rax; pop_rax] in
+    let/d asm1 := [storersp_rax; pop_rax] in
     let/d asm1 := List asm1 in
     let/d res := (asm1, l1) in
-    res
-  end.
+    res.
 
 (*
   RAX := RAX + top_of_stack
@@ -324,7 +349,9 @@ Definition c_store: asm_appl :=
   let/d add_rdi_rdx := ASMSyntax.Add RDI RDX in
   let/d store_rax_rdi := ASMSyntax.Store RAX RDI (word.of_Z (Z.of_nat 0)) in
   let/d pop_rax := ASMSyntax.Pop RAX in
-  let/d asm1 := [pop_rdi; pop_rdx; add_rdi_rdx; store_rax_rdi; pop_rax] in
+  let/d asm0 := [pop_rdi; pop_rdx; add_rdi_rdx; store_rax_rdi] in
+  let/d asm05 := [pop_rax] in
+  let/d asm1 := list_append asm0 asm05 in
   let/d res := List asm1 in
   res.
 
@@ -337,7 +364,8 @@ Fixpoint c_exp (e: exp) (l: nat) (vs: v_stack): asm_appl * nat :=
     let/d vs1 := None :: vs in
     let/d '(asm2, l2) := c_exp e2 l1 vs1 in
     let/d c_add_asm := c_add in
-    let/d asm_combined := asm1 +++ asm2 +++ c_add_asm in
+    let/d asm_combined0 := asm1 +++ asm2 in
+    let/d asm_combined := asm_combined0 +++ c_add_asm in
     let/d c_add_len := app_list_length c_add_asm in
     let/d l3 := l2 + c_add_len in
     let/d res := (asm_combined, l3) in
@@ -347,7 +375,8 @@ Fixpoint c_exp (e: exp) (l: nat) (vs: v_stack): asm_appl * nat :=
     let/d vs1 := None :: vs in
     let/d '(asm2, l2) := c_exp e2 l1 vs1 in
     let/d c_sub_asm := c_sub in
-    let/d asm_combined := asm1 +++ asm2 +++ c_sub_asm in
+    let/d asm_combined0 := asm1 +++ asm2 in
+    let/d asm_combined := asm_combined0 +++ c_sub_asm in
     let/d c_sub_len := app_list_length c_sub_asm in
     let/d l3 := l2 + c_sub_len in
     let/d res := (asm_combined, l3) in
@@ -356,8 +385,10 @@ Fixpoint c_exp (e: exp) (l: nat) (vs: v_stack): asm_appl * nat :=
     let/d '(asm1, l1) := c_exp e1 l vs in
     let/d vs1 := None :: vs in
     let/d '(asm2, l2) := c_exp e2 l1 vs1 in
-    let/d asm_combined := asm1 +++ asm2 +++ c_div in
-    let/d c_div_len := app_list_length c_div in
+    let/d asm_combined0 := asm1 +++ asm2 in
+    let/d cdiv := c_div in
+    let/d asm_combined := asm_combined0 +++ cdiv in
+    let/d c_div_len := app_list_length cdiv in
     let/d l3 := l2 + c_div_len in
     let/d res := (asm_combined, l3) in
     res
@@ -365,8 +396,10 @@ Fixpoint c_exp (e: exp) (l: nat) (vs: v_stack): asm_appl * nat :=
     let/d '(asm1, l1) := c_exp e1 l vs in
     let/d vs1 := None :: vs in
     let/d '(asm2, l2) := c_exp e2 l1 vs1 in
-    let/d asm_combined := asm1 +++ asm2 +++ c_load in
-    let/d c_load_len := app_list_length c_load in
+    let/d asm_combined0 := asm1 +++ asm2 in
+    let/d cload := c_load in
+    let/d asm_combined := asm_combined0 +++ cload in
+    let/d c_load_len := app_list_length cload in
     let/d l3 := l2 + c_load_len in
     let/d res := (asm_combined, l3) in
     res
@@ -396,8 +429,12 @@ Proof. unfold_fix_proof '@c_exps. Qed.
 *)
 Definition c_cmp (c: cmp) : cond :=
   match c with
-  | Less => ASMSyntax.Less RDI RBX
-  | Equal => ASMSyntax.Equal RDI RBX
+  | Less =>
+    let/d res := ASMSyntax.Less RDI RBX in
+    res
+  | Equal =>
+    let/d res := ASMSyntax.Equal RDI RBX in
+    res
   end.
 
 Fixpoint c_test_jump (t: test) (pos_label: nat) (neg_label: nat)
@@ -405,17 +442,25 @@ Fixpoint c_test_jump (t: test) (pos_label: nat) (neg_label: nat)
   match t with
   | Test c e1 e2 =>
     let/d '(asm1, l1) := c_exp e1 l vs in
-    let/d vs1 := None :: vs in
+    let/d none := None in
+    let/d vs1 := none :: vs in
     let/d '(asm2, l2) := c_exp e2 l1 vs1 in
-    let/d mov_rbx_rax := Mov RBX RAX in
-    let/d pop_rdi := Pop RDI in
-    let/d pop_rax := Pop RAX in
+    let/d rbx := RBX in
+    let/d rax := RAX in
+    let/d rdi := RDI in
+    let/d mov_rbx_rax := Mov rbx rax in
+    let/d pop_rdi := Pop rdi in
+    let/d pop_rax := Pop rax in
     let/d cmp_cond := c_cmp c in
     let/d jump_pos := ASMSyntax.Jump cmp_cond pos_label in
-    let/d jump_neg := ASMSyntax.Jump Always neg_label in
-    let/d c_cmp_list := [mov_rbx_rax; pop_rdi; pop_rax; jump_pos; jump_neg] in
+    let/d always := Always in
+    let/d jump_neg := ASMSyntax.Jump always neg_label in
+    let/d c_cmp_list1 := [mov_rbx_rax; pop_rdi; pop_rax; jump_pos] in
+    let/d c_cmp_list2 := [jump_neg] in
+    let/d c_cmp_list := list_append c_cmp_list1 c_cmp_list2 in
     let/d c_cmp_asm := List c_cmp_list in
-    let/d asm_combined := asm1 +++ asm2 +++ c_cmp_asm in
+    let/d asm_combined0 := asm1 +++ asm2 in
+    let/d asm_combined := asm_combined0 +++ c_cmp_asm in
     let/d c_cmp_len := app_list_length c_cmp_asm in
     let/d l3 := l2 + c_cmp_len in
     let/d res := (asm_combined, l3) in
@@ -425,11 +470,16 @@ Fixpoint c_test_jump (t: test) (pos_label: nat) (neg_label: nat)
     let/d l2_label := l + 2 in
     let/d '(asm1, l1) := c_test_jump t1 l1_label neg_label l2_label vs in
     let/d '(asm2, l2) := c_test_jump t2 pos_label neg_label l1 vs in
-    let/d jump_always_l2 := ASMSyntax.Jump Always l2_label in
-    let/d jump_to_start := List [jump_always_l2] in
-    let/d jump_always_l1 := ASMSyntax.Jump Always l1 in
-    let/d jump_to_t2 := List [jump_always_l1] in (* l1 is the start of t2*)
-    let/d asm_combined := jump_to_start +++ jump_to_t2 +++ asm1 +++ asm2 in
+    let/d always := Always in
+    let/d jump_always_l2 := ASMSyntax.Jump always l2_label in
+    let/d jump_to_start_list := [jump_always_l2] in
+    let/d jump_to_start := List jump_to_start_list in
+    let/d jump_always_l1 := ASMSyntax.Jump always l1 in
+    let/d jump_to_t2_list := [jump_always_l1] in (* l1 is the start of t2*)
+    let/d jump_to_t2 := List jump_to_t2_list in
+    let/d asm_combined0 := jump_to_start +++ jump_to_t2 in
+    let/d asm_combined1 := asm_combined0 +++ asm1 in
+    let/d asm_combined := asm_combined1 +++ asm2 in
     let/d res := (asm_combined, l2) in
     res
   | Or t1 t2 =>
@@ -437,11 +487,16 @@ Fixpoint c_test_jump (t: test) (pos_label: nat) (neg_label: nat)
     let/d l2_label := l + 2 in
     let/d '(asm1, l1) := c_test_jump t1 pos_label l1_label l2_label vs in
     let/d '(asm2, l2) := c_test_jump t2 pos_label neg_label l1 vs in
-    let/d jump_always_l2 := ASMSyntax.Jump Always l2_label in
-    let/d jump_to_start := List [jump_always_l2] in
-    let/d jump_always_l1 := ASMSyntax.Jump Always l1 in
-    let/d jump_to_t2 := List [jump_always_l1] in (* l1 is the start of t2*)
-    let/d asm_combined := jump_to_start +++ jump_to_t2 +++ asm1 +++ asm2 in
+    let/d always := Always in
+    let/d jump_always_l2 := ASMSyntax.Jump always l2_label in
+    let/d jump_to_start_list := [jump_always_l2] in
+    let/d jump_to_start := List jump_to_start_list in
+    let/d jump_always_l1 := ASMSyntax.Jump always l1 in
+    let/d jump_to_t2_list := [jump_always_l1] in (* l1 is the start of t2*)
+    let/d jump_to_t2 := List jump_to_t2_list in
+    let/d asm_combined0 := jump_to_start +++ jump_to_t2 in
+    let/d asm_combined1 := asm_combined0 +++ asm1 in
+    let/d asm_combined := asm_combined1 +++ asm2 in
     let/d res := (asm_combined, l2) in
     res
   | Not t' =>
@@ -479,50 +534,51 @@ Definition make_ret (vs: v_stack) (l: nat): asm_appl * nat :=
 passed to the function call *)
 Definition c_pops (xs: list exp) (vs: v_stack): asm_appl :=
   let/d k := list_length xs in
+  let/d rax := RAX in
+  let/d rdi := RDI in
+  let/d rdx := RDX in
+  let/d rbx := RBX in
+  let/d rbp := RBP in
   if k =? 0 then 
-    let/d push_rax := Push RAX in
+    let/d push_rax := Push rax in
     let/d asm_list := [push_rax] in
     let/d res := List asm_list in
     res
-  else
-  if k =? 1 then 
+  else if k =? 1 then 
     let/d empty_list := [] in
     let/d res := List empty_list in
     res
-  else
-  if k =? 2 then 
-    let/d pop_rdi := Pop RDI in
+  else if k =? 2 then 
+    let/d pop_rdi := Pop rdi in
     let/d asm_list := [pop_rdi] in
     let/d res := List asm_list in
     res
-  else
-  if k =? 3 then 
-    let/d pop_rdi := Pop RDI in
-    let/d pop_rdx := Pop RDX in
+  else if k =? 3 then 
+    let/d pop_rdi := Pop rdi in
+    let/d pop_rdx := Pop rdx in
     let/d asm_list := [pop_rdi; pop_rdx] in
     let/d res := List asm_list in
     res
-  else
-  if k =? 4 then 
-    let/d pop_rdi := Pop RDI in
-    let/d pop_rdx := Pop RDX in
-    let/d pop_rbx := Pop RBX in
+  else if k =? 4 then 
+    let/d pop_rdi := Pop rdi in
+    let/d pop_rdx := Pop rdx in
+    let/d pop_rbx := Pop rbx in
     let/d asm_list := [pop_rdi; pop_rdx; pop_rbx] in
     let/d res := List asm_list in
     res
-  else
-  if k =? 5 then 
-    let/d pop_rdi := Pop RDI in
-    let/d pop_rdx := Pop RDX in
-    let/d pop_rbx := Pop RBX in
-    let/d pop_rbp := Pop RBP in
+  else if k =? 5 then 
+    let/d pop_rdi := Pop rdi in
+    let/d pop_rdx := Pop rdx in
+    let/d pop_rbx := Pop rbx in
+    let/d pop_rbp := Pop rbp in
     let/d asm_list := [pop_rdi; pop_rdx; pop_rbx; pop_rbp] in
     let/d res := List asm_list in
     res
-  else 
+  else
     let/d even_xs := even_len xs in
     let/d give_up_label := give_up even_xs in
-    let/d jump_always := Jump Always give_up_label in
+    let/d always := Always in
+    let/d jump_always := Jump always give_up_label in
     let/d asm_list := [jump_always] in
     let/d res := List asm_list in
     res.
@@ -533,24 +589,27 @@ so the actual stack size is odd then)
 *)
 
 (** Builds a stack representation for parameters of a function *)
-Function call_v_stack (xs: list name) (acc: v_stack): v_stack :=
+Fixpoint call_v_stack (xs: list name) (acc: v_stack): v_stack :=
   match xs with
   | [] => acc
-  | x :: xs' => call_v_stack xs' (Some x :: acc)
+  | x :: xs' =>
+    let/d some_x := Some x in
+    let/d x_acc := some_x :: acc in
+    call_v_stack xs' x_acc
   end.
+Theorem call_v_stack_equation: ltac2:(unfold_fix_type '@call_v_stack).
+Proof. unfold_fix_proof '@call_v_stack. Qed.
 
 Definition c_pushes_vs (v_names: list name): list (option name) :=
-  match v_names with
-  | [] => 
+  let/d len := list_length v_names in
+  if len =? 0 then
     let/d none_val := None in
     let/d res := [none_val] in
     res
-  | _ => 
+  else
     let/d empty_list := @nil (option name) in
     let/d res := call_v_stack v_names empty_list in
-    res
-  end.
-
+    res.
 (** Push a list of variables onto the stack *)
 Definition c_pushes (v_names: list name) (l: nat): (asm_appl * v_stack * nat) :=
   let/d k := list_length v_names in
@@ -558,40 +617,41 @@ Definition c_pushes (v_names: list name) (l: nat): (asm_appl * v_stack * nat) :=
   if k =? 0 then 
     let/d empty_list := [] in
     let/d asm1 := List empty_list in
-    let/d res := (asm1, e, l) in
+    let/d pair1 := (asm1, e) in
+    let/d res := (pair1, l) in
     res
-  else
-  if k =? 1 then 
+  else if k =? 1 then 
     let/d empty_list := [] in
     let/d asm1 := List empty_list in
-    let/d res := (asm1, e, l) in
+    let/d pair1 := (asm1, e) in
+    let/d res := (pair1, l) in
     res
-  else
-  if k =? 2 then 
+  else if k =? 2 then 
     let/d push_rdi := Push RDI in
     let/d asm_list := [push_rdi] in
     let/d asm1 := List asm_list in
     let/d l1 := l + 1 in
-    let/d res := (asm1, e, l1) in
+    let/d pair1 := (asm1, e) in
+    let/d res := (pair1, l1) in
     res
-  else
-  if k =? 3 then 
+  else if k =? 3 then 
     let/d push_rdx := Push RDX in
     let/d push_rdi := Push RDI in
     let/d asm_list := [push_rdx; push_rdi] in
     let/d asm1 := List asm_list in
     let/d l1 := l + 2 in
-    let/d res := (asm1, e, l1) in
+    let/d pair1 := (asm1, e) in
+    let/d res := (pair1, l1) in
     res
-  else
-  if k =? 4 then 
+  else if k =? 4 then 
     let/d push_rbx := Push RBX in
     let/d push_rdx := Push RDX in
     let/d push_rdi := Push RDI in
     let/d asm_list := [push_rbx; push_rdx; push_rdi] in
     let/d asm1 := List asm_list in
     let/d l1 := l + 3 in
-    let/d res := (asm1, e, l1) in
+    let/d pair1 := (asm1, e) in
+    let/d res := (pair1, l1) in
     res
   else 
     let/d push_rbp := Push RBP in
@@ -601,7 +661,8 @@ Definition c_pushes (v_names: list name) (l: nat): (asm_appl * v_stack * nat) :=
     let/d asm_list := [push_rbp; push_rbx; push_rdx; push_rdi] in
     let/d asm1 := List asm_list in
     let/d l1 := l + 4 in
-    let/d res := (asm1, e, l1) in
+    let/d pair1 := (asm1, e) in
+    let/d res := (pair1, l1) in
     res.
 
 (* Call the given function, passing the arguments in registers*)
@@ -639,12 +700,15 @@ Fixpoint c_cmd (c: cmd) (l: nat) (fs: f_lookup) (vs: v_stack): (asm_appl * nat) 
     res
   | Update a e e' =>
     let/d '(asm1, l1) := c_exp a l vs in
-    let/d vs1 := None :: vs in
+    let/d none := None in
+    let/d vs1 := none :: vs in
     let/d '(asm2, l2) := c_exp e l1 vs1 in
-    let/d vs2 := None :: None :: vs in
+    let/d vs2 := none :: none :: vs in
     let/d '(asm3, l3) := c_exp e' l2 vs2 in
     let/d asm4 := c_store in
-    let/d asm_combined := asm1 +++ asm2 +++ asm3 +++ asm4 in
+    let/d asm_temp1 := asm1 +++ asm2 in
+    let/d asm_temp2 := asm_temp1 +++ asm3 in
+    let/d asm_combined := asm_temp2 +++ asm4 in
     let/d asm4_len := app_list_length asm4 in
     let/d l4 := l3 + asm4_len in
     let/d res := (asm_combined, l4) in
@@ -657,15 +721,25 @@ Fixpoint c_cmd (c: cmd) (l: nat) (fs: f_lookup) (vs: v_stack): (asm_appl * nat) 
     let/d '(asm2, l2) := c_cmd c1 l1 fs vs in
     let/d l2_plus1 := l2 + 1 in
     let/d '(asm3, l3) := c_cmd c2 l2_plus1 fs vs in
-    let/d jump_always_l3 := ASMSyntax.Jump Always l3_label in
-    let/d jump_to_test := List[jump_always_l3] in
-    let/d jump_always_l1 := ASMSyntax.Jump Always l1 in
-    let/d jump_to_c1 := List [jump_always_l1] in
-    let/d jump_always_l2_plus1 := ASMSyntax.Jump Always l2_plus1 in
-    let/d jump_to_c2 := List [jump_always_l2_plus1] in
-    let/d jump_always_l3_end := ASMSyntax.Jump Always l3 in
-    let/d jump_to_end := List [jump_always_l3_end] in
-    let/d asmres := jump_to_test +++ jump_to_c1 +++ jump_to_c2 +++ asm1 +++ asm2 +++ jump_to_end +++ asm3 in
+    let/d always := Always in
+    let/d jump_always_l3 := ASMSyntax.Jump always l3_label in
+    let/d jump_to_test_list := [jump_always_l3] in
+    let/d jump_to_test := List jump_to_test_list in
+    let/d jump_always_l1 := ASMSyntax.Jump always l1 in
+    let/d jump_to_c1_list := [jump_always_l1] in
+    let/d jump_to_c1 := List jump_to_c1_list in
+    let/d jump_always_l2_plus1 := ASMSyntax.Jump always l2_plus1 in
+    let/d jump_to_c2_list := [jump_always_l2_plus1] in
+    let/d jump_to_c2 := List jump_to_c2_list in
+    let/d jump_always_l3_end := ASMSyntax.Jump always l3 in
+    let/d jump_to_end_list := [jump_always_l3_end] in
+    let/d jump_to_end := List jump_to_end_list in
+    let/d asm_temp1 := jump_to_test +++ jump_to_c1 in
+    let/d asm_temp2 := asm_temp1 +++ jump_to_c2 in
+    let/d asm_temp3 := asm_temp2 +++ asm1 in
+    let/d asm_temp4 := asm_temp3 +++ asm2 in
+    let/d asm_temp5 := asm_temp4 +++ jump_to_end in
+    let/d asmres := asm_temp5 +++ asm3 in
     let/d res := (asmres, l3) in
     res
   | While tst body =>
@@ -674,16 +748,25 @@ Fixpoint c_cmd (c: cmd) (l: nat) (fs: f_lookup) (vs: v_stack): (asm_appl * nat) 
     let/d l3_label := l + 3 in
     let/d '(asm1, l1) := c_test_jump tst l1_label l2_label l3_label vs in
     let/d '(asm2, l2) := c_cmd body l1 fs vs in
-    let/d jump_always_l3 := ASMSyntax.Jump Always l3_label in
-    let/d jump_to_tst := List [jump_always_l3] in
-    let/d jump_always_l := ASMSyntax.Jump Always l in
-    let/d jump_to_beginning := List [jump_always_l] in
-    let/d jump_always_l1 := ASMSyntax.Jump Always l1 in
-    let/d jump_to_body := List [jump_always_l1] in
+    let/d always := Always in
+    let/d jump_always_l3 := ASMSyntax.Jump always l3_label in
+    let/d jump_to_tst_list := [jump_always_l3] in
+    let/d jump_to_tst := List jump_to_tst_list in
+    let/d jump_always_l := ASMSyntax.Jump always l in
+    let/d jump_to_beginning_list := [jump_always_l] in
+    let/d jump_to_beginning := List jump_to_beginning_list in
+    let/d jump_always_l1 := ASMSyntax.Jump always l1 in
+    let/d jump_to_body_list := [jump_always_l1] in
+    let/d jump_to_body := List jump_to_body_list in
     let/d l2_plus1 := l2 + 1 in
-    let/d jump_always_l2_plus1 := ASMSyntax.Jump Always l2_plus1 in
-    let/d jump_to_end := List [jump_always_l2_plus1] in
-    let/d asmres := jump_to_tst +++ jump_to_body +++ jump_to_end +++ asm1 +++ asm2 +++ jump_to_beginning in
+    let/d jump_always_l2_plus1 := ASMSyntax.Jump always l2_plus1 in
+    let/d jump_to_end_list := [jump_always_l2_plus1] in
+    let/d jump_to_end := List jump_to_end_list in
+    let/d asm_temp1 := jump_to_tst +++ jump_to_body in
+    let/d asm_temp2 := asm_temp1 +++ jump_to_end in
+    let/d asm_temp3 := asm_temp2 +++ asm1 in
+    let/d asm_temp4 := asm_temp3 +++ asm2 in
+    let/d asmres := asm_temp4 +++ jump_to_beginning in
     let/d res := (asmres, l2_plus1) in
     res
   | Call n f es =>
@@ -691,7 +774,8 @@ Fixpoint c_cmd (c: cmd) (l: nat) (fs: f_lookup) (vs: v_stack): (asm_appl * nat) 
     let/d '(asms, l1) := c_exps es l vs in
     let/d '(asm1, l2) := c_call vs target es l1 in
     let/d '(asm2, l3) := c_assign n l2 vs in
-    let/d asm_combined := asms +++ asm1 +++ asm2 in
+    let/d asm_temp1 := asms +++ asm1 in
+    let/d asm_combined := asm_temp1 +++ asm2 in
     let/d res := (asm_combined, l3) in
     res
   | Return e =>
@@ -706,7 +790,8 @@ Fixpoint c_cmd (c: cmd) (l: nat) (fs: f_lookup) (vs: v_stack): (asm_appl * nat) 
     let/d asm2_len := app_list_length asm2 in
     let/d l2 := l1 + asm2_len in
     let/d '(asm3, l3) := c_assign n l2 vs in
-    let/d asm_combined := asm1 +++ asm2 +++ asm3 in
+    let/d asm_temp1 := asm1 +++ asm2 in
+    let/d asm_combined := asm_temp1 +++ asm3 in
     let/d res := (asm_combined, l3) in
     res
   | GetChar n =>
@@ -722,7 +807,8 @@ Fixpoint c_cmd (c: cmd) (l: nat) (fs: f_lookup) (vs: v_stack): (asm_appl * nat) 
     let/d res := (asm_combined, l2) in
     res
   | Abort =>
-    let/d jump_always_abort := Jump Always abortLoc in
+    let/d always := Always in
+    let/d jump_always_abort := Jump always abortLoc in
     let/d asm_list := [jump_always_abort] in
     let/d asm1 := List asm_list in
     let/d l1 := l + 1 in
@@ -849,13 +935,22 @@ Definition c_declare_binders (v_names: list name) (c: cmd): (asm_appl * v_stack)
   let/d is_even := even_len vs_after_pushes in
   let/d none_val := None in
   let/d none_list := [none_val] in
-  let/d vs_binders1 := if is_even then list_append vs_binders none_list else vs_binders in
-  let/d binders1_len := list_length vs_binders1 in
-  let/d sub_rsp := Sub_RSP binders1_len in
-  let/d asm_list := [sub_rsp] in
-  let/d asm1 := List asm_list in
-  let/d res := (asm1, vs_binders1) in
-  res.
+  if is_even then
+    let/d vs_binders1 := list_append vs_binders none_list in
+    let/d binders1_len := list_length vs_binders1 in
+    let/d sub_rsp := Sub_RSP binders1_len in
+    let/d asm_list := [sub_rsp] in
+    let/d asm1 := List asm_list in
+    let/d res := (asm1, vs_binders1) in
+    res
+  else
+    let/d vs_binders1 := vs_binders in
+    let/d binders1_len := list_length vs_binders1 in
+    let/d sub_rsp := Sub_RSP binders1_len in
+    let/d asm_list := [sub_rsp] in
+    let/d asm1 := List asm_list in
+    let/d res := (asm1, vs_binders1) in
+    res.
 
 (** Compiles a single function definition into assembly code. *)
 Definition c_fundef (fundef: func) (l: nat) (fs: f_lookup): (asm_appl * nat) :=
@@ -867,17 +962,11 @@ Definition c_fundef (fundef: func) (l: nat) (fs: f_lookup): (asm_appl * nat) :=
     let/d '(asm1, vs1, l1) := c_pushes v_names l0 in
     let/d vs_combined := list_append vs1 vs_binders1 in
     let/d '(asm2, l2) := c_cmd body l1 fs vs_combined in
-    let/d asm_combined := asm0 +++ asm1 +++ asm2 in
+    let/d asm_temp1 := asm0 +++ asm1 in
+    let/d asm_combined := asm_temp1 +++ asm2 in
     let/d res := (asm_combined, l2) in
     res
   end.
-
-(* TODO: Can we use the same helper as with ASMToString.name2str? *)
-Definition name2str (n: N) (acc: string): string :=
-  let/d n_mod := N_modulo n 256 in
-  let/d ascii_val := ascii_of_N n_mod in
-  let/d res := String ascii_val acc in
-  res.
 
 Definition get_funcs (p: prog): list func :=
   match p with
@@ -895,23 +984,27 @@ Fixpoint c_fundefs (ds: list func) (l: nat) (fs: f_lookup): (asm_appl * list (na
   | [] => 
     let/d empty_list := [] in
     let/d asm1 := List empty_list in
-    let/d res := (asm1, fs, l) in
+    let/d pair1 := (asm1, fs) in
+    let/d res := (pair1, l) in
     res
   | d :: ds' =>
     let/d fname := name_of_func d in
-    (* TODO: is using name2str as a constant correct? Should we reify it?  *)
-    let/d empty_str := ""%string in
-    let/d fname_str := name2str fname empty_str in
+    (* TODO: removed the comment for now  *)
+    (* let/d empty_str := ""%string in
+    let/d fname_str := name2str fname in
     let/d comment_instr := Comment fname_str in
     let/d comment_list := [comment_instr] in
-    let/d comment := List comment_list in
-    let/d l_plus1 := l + 1 in
+    let/d comment := List comment_list in *)
+    let/d l_plus1 := l (* + 1 *) in
     let/d '(c1, l1) := c_fundef d l_plus1 fs in
-    let/d '(c2, fs', l2) := c_fundefs ds' l1 fs in
-    let/d asm_combined := comment +++ c1 +++ c2 in
+    let/d fundefs_result := c_fundefs ds' l1 fs in
+    let/d '(c2_fs_pair, l2) := fundefs_result in
+    let/d '(c2, fs') := c2_fs_pair in
+    let/d asm_combined := (* comment +++ *) c1 +++ c2 in
     let/d fname_pair := (fname, l_plus1) in
     let/d fs_new := fname_pair :: fs' in
-    let/d res := (asm_combined, fs_new, l2) in
+    let/d pair1 := (asm_combined, fs_new) in
+    let/d res := (pair1, l2) in
     res
   end.
 Theorem c_fundefs_equation: ltac2:(unfold_fix_type '@c_fundefs).
