coq/theories/automation/ToANF.v
@@ -1,0 +1,103 @@
+From Ltac2 Require Import Ltac2 Constr Std RedFlags.
+From impboot Require Import utils.Core.
+From impboot Require Import utils.AppList.
+From coqutil Require Import dlet.
+From coqutil Require Import Word.Interface.
+
+Ltac2 rec proper_const_f (c: constr): bool :=
+  match Constr.Unsafe.kind c with
+  (* | Var _ => true *)
+  (* TODO: probably should remove this (next) line – it allows too many undesirable things as consts *)
+  | Unsafe.Constant _ _ => true
+  | Unsafe.Constructor _ _ => true
+  | Unsafe.App c cs => Bool.and (proper_const_f c) (Array.for_all proper_const_f cs)
+  | _ => false
+  end.
+Ltac2 proper_const (c: constr): bool :=
+  let evaluated := eval_cbv beta c in
+  proper_const_f evaluated.
+
+Ltac2 rec is_allowed (c: constr): bool :=
+  match! c with
+  | word.of_Z ?c1 => is_allowed c1
+  | Z.of_nat ?c1 => is_allowed c1
+  | Z.of_N ?c1 => is_allowed c1
+  | N.to_nat ?c1 => is_allowed c1
+  | N.of_nat ?c1 => is_allowed c1
+  | _ => proper_const c
+  end.
+
+(* Converts an expression to ANF-like form, such that every function call,
+constructor call, operation is let bound and never nested. The allowed top level
+expressions are matches, ifs, let bindings, and simple expressions in return
+positions. All if conditions can be assumed to be correct. *)
+(* e.g.
+  f (1 + 2) (g 3)
+  ===>
+  let a := 1 + 2 in
+  let b := g 3 in
+  let c := f a b in
+  c
+
+  if a <? b then
+    h (a + 1)
+  else
+    h (b + 1)
+  ===>
+  if a <? b then
+    let d := a + 1 in
+    let e := h d in
+    e
+  else
+    let d := b + 1 in
+    let e := h d in
+    e
+
+  let x := f (1 + 2) (g 3) in
+  x + 1
+  ===>
+  let a := 1 + 2 in
+  let b := g 3 in
+  let c := f a b in
+  let d := c + 1 in
+  d
+*)
+Ltac2 rec to_anf (e: constr): constr :=
+  match! e with
+  | let/d x := ?e1 in ?e2 =>
+    let e1_anf := to_anf e1 in
+    let e2_anf := to_anf e2 in
+    constr:(let/d x := $e1_anf in $e2_anf)
+  | if ?cond then ?then_branch else ?else_branch =>
+    let cond_anf := to_anf cond in
+    let then_anf := to_anf then_branch in
+    let else_anf := to_anf else_branch in
+    constr:(if $cond_anf then $then_anf else $else_anf)
+  | match ?_scrut with _ => _ end =>
+    e (* TODO *)
+  | ?f ?arg1 ?arg2 =>
+    let arg1_anf := to_anf arg1 in
+    let arg2_anf := to_anf arg2 in
+    let tmp1 := Fresh.in_goal (Option.get (Ident.of_string "anf_tmp")) in
+    let tmp1_constr := Unsafe.make (Unsafe.Var tmp1) in
+    let tmp2 := Fresh.in_goal (Option.get (Ident.of_string "anf_tmp")) in
+    let tmp2_constr := Unsafe.make (Unsafe.Var tmp2) in
+    let f_anf := to_anf constr:($f $tmp1_constr $tmp2_constr) in
+    constr:(let/d tmp1 := $arg1_anf in
+            let/d tmp2 := $arg2_anf in
+            let res := $f_anf in
+            res)
+  | ?f ?arg =>
+    let arg_anf := to_anf arg in
+    let tmp := Fresh.in_goal (Option.get (Ident.of_string "anf_tmp")) in
+    let tmp_constr := Unsafe.make (Unsafe.Var tmp) in
+    let f_anf := to_anf constr:($f $tmp_constr) in
+    constr:(let tmp := $arg_anf in
+            let res := $f_anf in
+            res)
+  | _ =>
+    e
+  end.
+
+(* split strings to intermediate lets *)
+(* split lists to intermediate lets *)
