coq/theories/automation/ToLowerable.v
@@ -1,0 +1,97 @@
+From Ltac2 Require Import Ltac2 Constr Std RedFlags.
+From impboot Require Import utils.Core.
+From impboot Require Import utils.AppList.
+From coqutil Require Import dlet.
+From coqutil Require Import Word.Interface.
+From impboot Require Import
+  commons.CompilerUtils
+  automation.ToANF.
+
+(* rewrite every N.mul to mul_N call and every Nat.mul to nat_mul call *)
+
+Lemma dlet_spec: forall {A B: Type} (a: A) (f: A -> B),
+  let/d x := a in f x = let x := a in f x.
+Proof.
+  intros; reflexivity ().
+Qed.
+
+Lemma split_string: forall {A} (c1 c2 c3 c4 c5: ascii) (s: string) (k: string -> A),
+  (let/d str1 := String c1 (String c2 (String c3 (String c4 (String c5 s)))) in k str1) =
+  let/d str_front := String c1 (String c2 (String c3 (String c4 EmptyString))) in
+  let/d str_rest := String c5 s in
+  let/d str1 := append str_front str_rest in
+  k str1.
+Proof.
+  intros; reflexivity ().
+Qed.
+
+Lemma split_list: forall {A B} (e1 e2 e3 e4 e5: A) (l: list A) (k: list A -> B),
+  (let/d l1 := e1 :: e2 :: e3 :: e4 :: e5 :: l in k l1) =
+  let/d l_front := e1 :: e2 :: e3 :: e4 :: [] in
+  let/d l_rest := e5 :: l in
+  let/d l1 := l_front ++ l_rest in
+  k l1.
+Proof.
+  intros; reflexivity ().
+Qed.
+
+Ltac2 rewrite_lowerable () :=
+  repeat (match! goal with
+  | [ |- context [ N.mul _ _ ] ] =>
+    rewrite <- mul_N_spec
+  | [ |- context [ Nat.mul _ _ ] ] =>
+    rewrite <- mul_nat_spec
+  | [ |- context [ append _ _ ] ] =>
+    rewrite <- string_append_spec
+  | [ |- context [ List.app _ _ ] ] =>
+    rewrite <- list_append_spec
+  | [ |- context [ List.length _ ] ] =>
+    rewrite <- list_length_spec
+  | [ |- context [
+    let/d x := (String _ (String _ (String _ (String _ (String _ _))))) in _ ] ] =>
+    rewrite split_string
+  | [ |- context [
+    let/d x := (_ :: _ :: _ :: _ :: _ :: _) in _ ] ] =>
+    rewrite split_list
+  end).
+
+(* test *)
+
+Definition test1 (a b: N): N :=
+  a * b + N.mul b a.
+
+Goal forall (a b: N), test1 a b = test1 a b.
+  intros; unfold test1.
+  rewrite_lowerable ().
+  reflexivity ().
+Qed.
+
+Definition test2 (a b: N): N :=
+  let/d d_div_a := N.mul b a in
+  (a * b + d_div_a)%N.
+
+Goal forall (a b: N), test2 a b = test2 a b.
+  intros; unfold test2.
+  rewrite_lowerable ().
+  reflexivity ().
+Qed.
+
+Definition test_split_string (s1 s2: string): string :=
+  let/d s := "abcdefg"%string in
+  append s s2.
+
+Goal forall (s1 s2: string), test_split_string s1 s2 = test_split_string s1 s2.
+  intros; unfold test_split_string.
+  rewrite_lowerable ().
+  reflexivity ().
+Qed.
+
+Definition test_split_list (l1 l2: list nat): list nat :=
+  let/d l := [1;2;3;4;5;6;7] in
+  l ++ l2.
+
+Goal forall (l1 l2: list nat), test_split_list l1 l2 = test_split_list l1 l2.
+  intros; unfold test_split_list.
+  rewrite_lowerable ().
+  reflexivity ().
+Qed.
