coq/theories/derivations/CompilerDerivations.v
@@ -1,0 +1,271 @@
+From impboot Require Import utils.Core.
+From impboot Require Import utils.Llist.
+Import Llist.
+From impboot Require Import utils.AppList.
+From impboot Require Import commons.ProofUtils.
+Require Import impboot.assembly.ASMSyntax.
+Require Import impboot.assembly.ASMToString.
+Require Import impboot.imperative.ImpSyntax.
+Require Import impboot.utils.AppList.
+Require Import impboot.parsing.Parser.
+Require Import impboot.imp2asm.ImpToASMCodegen.
+Require Import impboot.imp2asm.Compiler.
+From impboot Require Import automation.Ltac2Utils.
+From impboot Require Import commons.CompilerUtils.
+From impboot Require Import functional.FunValues.
+From impboot Require Import functional.FunSemantics.
+Require Import impboot.automation.RelCompiler.
+Require Import impboot.automation.ltac2.UnfoldFix.
+Require Import impboot.automation.AutomationLemmas.
+Require Import coqutil.Word.Interface.
+Require Import ZArith.
+From Stdlib Require Import FunInd.
+From Stdlib Require Import derive.Derive.
+From Stdlib Require Import Lia.
+From Ltac2 Require Import Ltac2.
+
+From impboot Require Import derivations.AsmToStringDerivations.
+From impboot Require Import derivations.ParserDerivations.
+From impboot Require Import derivations.ImpToASMCodegenDerivations.
+From impboot Require Import derivations.CompilerUtilsDerivations.
+
+Derive compiler_prog
+  in ltac2:(relcompile_tpe 'compiler_prog 'compiler ['str2imp; 'codegen; 'asm2str])
+  as compiler_prog_proof.
+Proof.
+  time relcompile.
+Qed.
+
+Definition read_inp_prog: FunSyntax.defun :=
+  FunSyntax.Defun (name_enc "read_inp") ([] : list N)
+    (
+      FunSyntax.Let (name_enc "curr") (FunSyntax.Op FunSyntax.Read []) (
+        FunSyntax.If FunSyntax.Equal [FunSyntax.Var (name_enc "curr"); FunSyntax.Const (2 ^ 32 - 1)%N] 
+          (FunSyntax.Const 0) (
+            FunSyntax.Let (name_enc "rest") (FunSyntax.Call (name_enc "read_inp") ([] : list FunSyntax.exp)) (
+              FunSyntax.Let (name_enc "result") (FunSyntax.Op FunSyntax.Cons [FunSyntax.Var (name_enc "curr"); FunSyntax.Var (name_enc "rest")])
+                (FunSyntax.Var (name_enc "result"))
+            )
+          )
+      )
+    ).
+
+Theorem read_inp_fn_thm:
+  ∀ body : FunSyntax.exp,
+    read_inp_prog = FunSyntax.Defun (name_enc "read_inp") ([] : list N) body →
+  ∀ (inp: list ascii) (s: state),
+    s.(input) = of_list inp →
+    lookup_fun (name_enc "read_inp") (funs s) = Some ([] : list N, body) →
+    eval_app (name_enc "read_inp") [] s (encode inp, set_input s Lnil).
+Proof.
+  intros * Hfneq.
+  induction inp as [| a inp IH]; intros.
+  all: eapply trans_app; eauto.
+  2,4: reflexivity.
+  all: inversion Hfneq; clear H1.
+  all: unfold make_env.
+  1: { (* empty input *)
+    inversion H; subst; simpl.
+    econstructor.
+    1: repeat econstructor.
+    1: simpl; unfold next; rewrite H3; reflexivity.
+    destruct s; unfold set_input; simpl.
+    repeat econstructor.
+  }
+  (* non-empty input *)
+  inversion H; subst; simpl.
+  econstructor.
+  1: repeat econstructor.
+  1: simpl; unfold next; rewrite H3; reflexivity.
+  econstructor.
+  1: repeat econstructor.
+  1: econstructor.
+  specialize N_ascii_bounded with (a := a) as Habounded.
+  assert (N_of_ascii a <> (2 ^ 32 - 1)%N) as Hneq by ltac1:(lia); rewrite <- N.eqb_neq in Hneq; simpl in Hneq.
+  rewrite Hneq.
+  econstructor.
+  1: {
+    eapply trans_Call.
+    1: repeat econstructor.
+    eapply IH; eauto.
+  }
+  repeat econstructor.
+Qed.
+
+Definition print_string_prog: FunSyntax.defun :=
+  FunSyntax.Defun (name_enc "print_string") [name_enc "str"] (
+    FunSyntax.If FunSyntax.Equal [FunSyntax.Var (name_enc "str"); FunSyntax.Const 0]
+      (FunSyntax.Const 0) (
+        FunSyntax.Let (name_enc "head") (FunSyntax.Op FunSyntax.Head [FunSyntax.Var (name_enc "str")]) (
+          FunSyntax.Let (name_enc "tail") (FunSyntax.Op FunSyntax.Tail [FunSyntax.Var (name_enc "str")]) (
+            FunSyntax.Let (name_enc "write_res") (FunSyntax.Op FunSyntax.Write [FunSyntax.Var (name_enc "head")]) (
+              FunSyntax.Call (name_enc "print_string") [FunSyntax.Var (name_enc "tail")]
+            )
+          )
+        )
+      )
+  ).
+
+Theorem print_string_thm:
+  ∀ body : FunSyntax.exp,
+    print_string_prog = FunSyntax.Defun (name_enc "print_string") [name_enc "str"] body →
+  ∀ (str: string) (s: state),
+    lookup_fun (name_enc "print_string") (funs s) = Some ([name_enc "str"], body) →
+    eval_app (name_enc "print_string") [encode str] s (Num 0, set_output s (s.(output) ++ str)).
+Proof.
+  intros * Hfneq.
+  induction str.
+  (* TODO: fix didn't work *)
+  (* ltac1:(fix IH 2). *)
+  all: intros.
+  all: eapply trans_app; eauto.
+  2,4: reflexivity.
+  all: inversion Hfneq; clear H1.
+  all: unfold make_env.
+  (* destruct str; simpl. *)
+  1: { (* empty string *)
+    econstructor.
+    1: repeat econstructor.
+    1: econstructor.
+    simpl.
+    destruct s; unfold set_output; rewrite string_app_r_nil; simpl.
+    econstructor.
+  }
+  (* non-empty string *)
+  econstructor.
+  1: repeat econstructor.
+  1: econstructor.
+  simpl.
+  econstructor.
+  1: econstructor.
+  1: econstructor; eauto with fenvDb.
+  1: econstructor.
+  econstructor.
+  1: {
+    econstructor.
+    1: repeat econstructor.
+    econstructor.
+  }
+  econstructor.
+  1: {
+    econstructor.
+    1: repeat econstructor.
+    ltac1:(with_strategy transparent [encode] simpl encode).
+    simpl; unfold enc_char.
+    specialize N_ascii_bounded with (a := a) as Habounded; rewrite <- N.ltb_lt in Habounded.
+    rewrite Habounded.
+    econstructor.
+  }
+  1: eapply trans_Call.
+  1: repeat econstructor.
+  set (s1 := set_output s (s.(output) ++ String a "")).
+  unfold set_output in *; simpl in *.
+  unfold enc_char in *; rewrite ascii_N_embedding in *.
+  assert (s.(output) ++ String a EmptyString ++ str = s.(output) ++ String a str) as <-.
+  1: rewrite string_cons_nil_app; reflexivity.
+  rewrite string_app_assoc.
+  destruct s; simpl in *.
+  eapply IHstr; eauto.
+  (* apply IH with (1 := Hstrlt) (2 := H0) (str := str) (s := s1). *)
+Qed.
+
+Theorem compiler_thm:
+  ∀ (s: state) (inp: list ascii),
+    (∀ fname args fn,
+      In (FunSyntax.Defun fname args fn) ([compiler_prog] ++ ImpToASMCodegen_funs ++ ASMToString_funs ++ ParserDerivations_funs ++ CompilerUtils_funs) →
+      lookup_fun fname (funs s) = Some (args, fn)) ->
+    eval_app (name_enc "compiler") [encode inp] s ((encode (compiler inp)), s).
+Proof.
+  intros * Hlookup_fun.
+  eapply compiler_prog_proof; eauto; try reflexivity.
+  4: eapply Hlookup_fun; simpl; left; reflexivity.
+  1: {
+    intros; eapply str2imp_thm; eauto; try reflexivity.
+    intros; eapply Hlookup_fun; eapply in_or_app; right; eapply in_or_app; right; eapply in_or_app; right; eauto.
+  }
+  1: {
+    intros; eapply codegen_thm; eauto; try reflexivity.
+    intros; eapply Hlookup_fun; eapply in_or_app; right; eapply in_app_or in H; destruct H; eauto.
+    1: eapply in_or_app; left; eauto.
+    1: eapply in_or_app; right; eapply in_or_app; right; eapply in_or_app; right; eauto.
+  }
+  intros; eapply asm2str_thm; eauto; try reflexivity.
+  intros; eapply Hlookup_fun; eapply in_or_app; right; eapply in_or_app; right; eapply in_app_or in H; destruct H; eauto.
+  1: eapply in_or_app; left; eauto.
+  1: eapply in_or_app; right; eapply in_or_app; right; eauto.
+Qed.
+
+Definition compiler_main: FunSyntax.exp := (
+  FunSyntax.Let (name_enc "inp") (FunSyntax.Call (name_enc "read_inp") ([] : list FunSyntax.exp)) (
+    FunSyntax.Let (name_enc "out_str") (FunSyntax.Call (name_enc "compiler") [FunSyntax.Var (name_enc "inp")]) (
+      FunSyntax.Call (name_enc "print_string") [FunSyntax.Var (name_enc "out_str")]
+    )
+  )
+).
+
+Definition compiler_funs: list FunSyntax.defun :=
+  [compiler_prog] ++ ImpToASMCodegen_funs ++ ASMToString_funs ++ ParserDerivations_funs ++ CompilerUtils_funs.
+
+Definition compiler_program_prog: FunSyntax.prog :=
+  FunSyntax.Program (read_inp_prog :: print_string_prog :: compiler_funs) compiler_main.
+
+Lemma In_IMP_lookup_fun:
+  forall fname args fn fns,
+    In (FunSyntax.Defun fname args fn) fns →
+    NoDup (List.map (fun d => match d with FunSyntax.Defun name _ _ => name end) fns) ->
+    lookup_fun fname fns = Some (args, fn).
+Proof.
+  intros * HIn HNoDup.
+  induction fns; simpl in *; try ltac1:(try contradiction).
+  destruct HIn; subst; simpl.
+  1: rewrite N.eqb_refl; reflexivity.
+  destruct a; inversion HNoDup; subst; clear HNoDup.
+  destruct (_ =? _)%N eqn:?; simpl in *.
+  2: eapply IHfns; eauto.
+  1: rewrite N.eqb_eq in Heqb; subst; simpl.
+  eapply in_map with (f := fun d => match d with FunSyntax.Defun name _ _ => name end) in H.
+  ltac1:(contradiction).  
+Qed.
+
+Lemma noDup_all_funs:
+  NoDup (List.map (λ d : FunSyntax.defun, match d with
+    | FunSyntax.Defun name _ _ => name
+    end) (read_inp_prog :: print_string_prog :: compiler_funs)).
+Proof.
+Admitted.
+
+Theorem compiler_program_thm:
+  ∀ inp,
+    prog_terminates (of_list inp) compiler_program_prog (compiler inp).
+Proof.
+  intros.
+  unfold prog_terminates, init_state, FunSyntax.get_defs, FunSyntax.get_main.
+  do 2 eexists.
+  split.
+  2: ltac1:(shelve).
+  Opaque compiler_funs.
+  unfold compiler_program_prog.
+  unfold compiler_main.
+  econstructor.
+  1: {
+    eapply trans_Call.
+    1: repeat econstructor.
+    eapply read_inp_fn_thm; simpl; eauto; try reflexivity.
+  }
+  unfold set_input; simpl.
+  econstructor.
+  1: {
+    eapply trans_Call.
+    1: repeat econstructor.
+    eapply compiler_thm; eauto; try reflexivity.
+    intros; eapply In_IMP_lookup_fun.
+    1: simpl; right; right; eauto.
+    simpl.
+    eapply noDup_all_funs.
+  }
+  eapply trans_Call.
+  1: repeat econstructor.
+  eapply print_string_thm; eauto; try reflexivity.
+  Unshelve.
+  simpl; reflexivity.
+Qed.
