coq/theories/derivations/CompilerUtilsDerivations.v
@@ -1,0 +1,168 @@
+From impboot Require Import utils.Core.
+From impboot Require Import utils.AppList.
+Require Import impboot.assembly.ASMSyntax.
+Require Import impboot.assembly.ASMToString.
+Require Import impboot.imperative.ImpSyntax.
+Require Import impboot.utils.AppList.
+Require Import impboot.imp2asm.ImpToASMCodegen.
+Require Import impboot.commons.CompilerUtils.
+From impboot Require Import automation.Ltac2Utils.
+From impboot Require Import commons.CompilerUtils.
+From impboot Require Import functional.FunValues.
+From impboot Require Import functional.FunSemantics.
+Require Import impboot.automation.RelCompiler.
+Require Import impboot.automation.ltac2.UnfoldFix.
+Require Import impboot.automation.AutomationLemmas.
+Require Import coqutil.Word.Interface.
+Require Import ZArith.
+From Stdlib Require Import FunInd.
+From Stdlib Require Import derive.Derive.
+From Stdlib Require Import Lia.
+From Ltac2 Require Import Ltac2.
+
+Derive nat_modulo_prog
+  in ltac2:(relcompile_tpe 'nat_modulo_prog 'nat_modulo ['mul_nat]) 
+  as nat_modulo_prog_proof.
+Proof.
+  time relcompile.
+  ltac1:(lia).
+Qed.
+
+Derive N_modulo_prog
+  in ltac2:(relcompile_tpe 'N_modulo_prog 'N_modulo ['mul_N]) 
+  as N_modulo_prog_proof.
+Proof.
+  time relcompile.
+  ltac1:(lia).
+Qed.
+
+Theorem string_append_equation: ltac2:(unfold_fix_type '@string_append).
+Proof. unfold_fix_proof '@string_append. Qed.
+Derive string_append_prog
+  in ltac2:(relcompile_tpe 'string_append_prog 'string_append [])
+  as string_append_prog_proof.
+Proof.
+  time relcompile.
+Qed.
+
+Theorem num2str_f_equation: ltac2:(unfold_fix_type '@num2str_f).
+Proof. unfold_fix_proof '@num2str_f. Qed.
+
+Derive num2str_f_prog
+  in ltac2:(relcompile_tpe 'num2str_f_prog 'num2str_f ['nat_modulo])
+  as num2str_f_prog_proof.
+Proof.
+  time relcompile.
+  all: ltac1:(try lia).
+  all: subst; specialize nat_modulo_le with (n := n) (m := 10); ltac1:(lia).
+Qed.
+
+Derive num2str_prog
+  in ltac2:(relcompile_tpe 'num2str_prog 'num2str ['num2str_f])
+  as num2str_prog_proof.
+Proof.
+  time relcompile.
+Qed.
+
+Theorem N2str_f_equation: ltac2:(unfold_fix_type '@N2str_f).
+Proof. unfold_fix_proof '@N2str_f. Qed.
+
+Derive N2str_f_prog
+  in ltac2:(relcompile_tpe 'N2str_f_prog 'N2str_f ['N_modulo])
+  as N2str_f_prog_proof.
+Proof.
+  time relcompile.
+  all: ltac1:(try lia).
+  all: rewrite ?N.ltb_lt in *; ltac1:(try lia).
+  all: subst; specialize N_modulo_le with (n := n) (m := 10%N) as ?; ltac1:(try lia).
+Qed.
+
+Derive N2str_prog
+  in ltac2:(relcompile_tpe 'N2str_prog 'N2str ['N2str_f])
+  as N2str_prog_proof.
+Proof.
+  time relcompile.
+  ltac1:(try lia).
+Qed.
+
+Theorem list_length_equation: ltac2:(unfold_fix_type '@list_length).
+Proof. unfold_fix_proof '@list_length. Qed.
+
+Derive list_length_prog
+  in ltac2:(relcompile_tpe 'list_length_prog '@list_length [])
+  as list_length_prog_proof.
+Proof.
+  time relcompile.
+Qed.
+
+Theorem list_append_equation: ltac2:(unfold_fix_type '@list_append).
+Proof. unfold_fix_proof '@list_append. Qed.
+
+Derive list_append_prog
+  in ltac2:(relcompile_tpe 'list_append_prog '@list_append [])
+  as list_append_prog_proof.
+Proof.
+  time relcompile.
+Qed.
+
+Theorem flatten_equation: ltac2:(unfold_fix_type '@flatten).
+Proof. unfold_fix_proof '@flatten. Qed.
+
+Derive flatten_prog
+  in ltac2:(relcompile_tpe 'flatten_prog '@flatten ['@list_append])
+  as flatten_prog_proof.
+Proof.
+  time relcompile.
+Qed.
+
+Theorem app_list_length_equation: ltac2:(unfold_fix_type '@app_list_length).
+Proof. unfold_fix_proof '@app_list_length. Qed.
+
+Derive app_list_length_prog
+  in ltac2:(relcompile_tpe 'app_list_length_prog '@app_list_length ['@list_length])
+  as app_list_length_prog_proof.
+Proof.
+  time relcompile.
+Qed.
+
+Theorem mul_nat_equation: ltac2:(unfold_fix_type '@mul_nat).
+Proof. unfold_fix_proof '@mul_nat. Qed.
+Derive mul_nat_prog
+  in ltac2:(relcompile_tpe 'mul_nat_prog 'mul_nat [])
+  as mul_nat_prog_proof.
+Proof.
+  time relcompile.
+Qed.
+
+Theorem mul_N_f_equation: ltac2:(unfold_fix_type '@mul_N_f).
+Proof. unfold_fix_proof '@mul_N_f. Qed.
+Derive mul_N_f_prog
+  in ltac2:(relcompile_tpe 'mul_N_f_prog 'mul_N_f [])
+  as mul_N_f_prog_proof.
+Proof.
+  time relcompile.
+Qed.
+
+Derive mul_N_prog
+  in ltac2:(relcompile_tpe 'mul_N_prog 'mul_N ['mul_N_f])
+  as mul_N_prog_proof.
+Proof.
+  time relcompile.
+Qed.
+
+Definition CompilerUtils_funs := [
+  mul_nat_prog;
+  mul_N_f_prog;
+  mul_N_prog;
+  nat_modulo_prog;
+  N_modulo_prog;
+  num2str_f_prog;
+  num2str_prog;
+  N2str_f_prog;
+  N2str_prog;
+  list_length_prog;
+  list_append_prog;
+  flatten_prog;
+  app_list_length_prog;
+  string_append_prog
+].
