coq/theories/utils/Core.v
@@ -24,106 +24,20 @@ Notation "'let/d' x := val 'in' body" :=
 Notation
   "'let/d' ''(' x , y ')' := val 'in' body" :=
   (dlet val (fun v =>
-      let x := fst v in
-      let y := snd v in
+      let/d x := fst v in
+      let/d y := snd v in
       body))
   (at level 200, body at level 200, only parsing).
 
 Notation
   "'let/d' ''(' x , y , z ')' := val 'in' body" :=
   (dlet val (fun v =>
-      let x := fst (fst v) in
-      let y := snd (fst v) in
-      let z := snd v in
+      let/d fst_v := fst v in
+      let/d x := fst fst_v in
+      let/d y := snd fst_v in
+      let/d z := snd v in
       body))
   (at level 200, body at level 200, only parsing).
-
-(* CASE *)
-
-Class Analyzable T :=
-  { R: Type; analyze: T -> R }.
-
-Definition list_CASE [A] (l : list A) [B] (fnil : B) (fcons : A -> list A -> B) : B :=
-  match l with
-  | [] => fnil
-  | x :: xs => fcons x xs
-  end.
-
-Instance Analyzable_List A : Analyzable (list A) :=
-  {
-    R := forall B, B -> (A -> list A -> B) -> B;
-    analyze l _ fnil fcons :=
-      match l with
-      | [] => fnil
-      | x :: xs => fcons x xs
-      end
-  }.
-
-Definition option_CASE [A] (o : option A) [B] (fnone : B) (fsome : A -> B) : B :=
-  match o with
-  | None => fnone
-  | Some x => fsome x
-  end.
-
-Instance Analyzable_Option A : Analyzable (option A) :=
-  {
-    R := forall B, B -> (A -> B) -> B;
-    analyze o _ fnone fsome :=
-      match o with
-      | None => fnone
-      | Some x => fsome x
-      end
-  }.
-
-Definition pair_CASE [A1 A2] (p : A1 * A2) [B] (f: A1 -> A2 -> B) : B :=
-  match p with
-  | (x, y) => f x y
-  end.
-
-Instance Analyzable_Pair A1 A2 : Analyzable (A1 * A2) :=
-  {
-    R := forall B, (A1 -> A2 -> B) -> B;
-    analyze p _ f :=
-      match p with
-      | (x, y) => f x y
-      end
-  }.
-
-Definition nat_CASE (n : nat) [A] (f0 : A) (fS : nat -> A) : A :=
-  match n with
-  | 0 => f0
-  | S n' => fS n'
-  end.
-
-Instance Analyzable_Nat : Analyzable nat :=
-  {
-    R := forall A, A -> (nat -> A) -> A;
-    analyze n _ f0 fS :=
-      match n with
-      | 0 => f0
-      | S n' => fS n'
-      end
-  }.
-
-(* FIX *)
-
-Fixpoint fold_right {A B} (f : B -> A -> A) (acc : A) (l : list B) : A :=
-  match l with
-  | nil => acc
-  | x :: xs =>
-    f x (fold_right f acc xs)
-  end.
-
-(* TODO(kπ) check this *)
-Definition fold_left {A B} (f : A -> B -> A) (acc : A) (l : list B) : A :=
-  fold_right (fun x g => fun z => g (f z x)) (fun z => z) l acc.
-
-Fixpoint nat_FIX {A C} (n : nat) (f0 : C -> A) (fS : (C -> A) -> nat -> C -> A) : C -> A :=
-  match n with
-  | 0 => f0
-  | S n' =>
-    fS (nat_FIX n' f0 fS) n'
-  end.
 
 (* Word *)
 
